<?xml version="1.0" encoding="UTF-8"?>
<!DOCTYPE rdf:RDF [
	<!ENTITY dct "http://purl.org/dc/terms/">
	<!ENTITY fibo-fnd-aap-agt "https://spec.edmcouncil.org/fibo/ontology/FND/AgentsAndPeople/Agents/">
	<!ENTITY fibo-fnd-aap-ppl "https://spec.edmcouncil.org/fibo/ontology/FND/AgentsAndPeople/People/">
	<!ENTITY fibo-fnd-arr-cls "https://spec.edmcouncil.org/fibo/ontology/FND/Arrangements/ClassificationSchemes/">
	<!ENTITY fibo-fnd-arr-lif "https://spec.edmcouncil.org/fibo/ontology/FND/Arrangements/Lifecycles/">
	<!ENTITY fibo-fnd-dt-fd "https://spec.edmcouncil.org/fibo/ontology/FND/DatesAndTimes/FinancialDates/">
	<!ENTITY fibo-fnd-dt-oc "https://spec.edmcouncil.org/fibo/ontology/FND/DatesAndTimes/Occurrences/">
	<!ENTITY fibo-fnd-gao-obj "https://spec.edmcouncil.org/fibo/ontology/FND/GoalsAndObjectives/Objectives/">
	<!ENTITY fibo-fnd-org-fm "https://spec.edmcouncil.org/fibo/ontology/FND/Organizations/FormalOrganizations/">
	<!ENTITY fibo-fnd-plc-loc "https://spec.edmcouncil.org/fibo/ontology/FND/Places/Locations/">
	<!ENTITY fibo-fnd-pty-pty "https://spec.edmcouncil.org/fibo/ontology/FND/Parties/Parties/">
	<!ENTITY fibo-fnd-pty-rl "https://spec.edmcouncil.org/fibo/ontology/FND/Parties/Roles/">
	<!ENTITY fibo-fnd-qt-qtu "https://spec.edmcouncil.org/fibo/ontology/FND/Quantities/QuantitiesAndUnits/">
	<!ENTITY fibo-fnd-rel-rel "https://spec.edmcouncil.org/fibo/ontology/FND/Relations/Relations/">
	<!ENTITY fibo-fnd-utl-alx "https://spec.edmcouncil.org/fibo/ontology/FND/Utilities/Analytics/">
	<!ENTITY fibo-fnd-utl-av "https://spec.edmcouncil.org/fibo/ontology/FND/Utilities/AnnotationVocabulary/">
	<!ENTITY lcc-cr "https://www.omg.org/spec/LCC/Countries/CountryRepresentation/">
	<!ENTITY lcc-lr "https://www.omg.org/spec/LCC/Languages/LanguageRepresentation/">
	<!ENTITY oe2020-pkm-mvs "https://tw.rpi.edu/ontology-engineering/oe2020/pokemon-moveset/">
	<!ENTITY owl "http://www.w3.org/2002/07/owl#">
	<!ENTITY rdf "http://www.w3.org/1999/02/22-rdf-syntax-ns#">
	<!ENTITY rdfs "http://www.w3.org/2000/01/rdf-schema#">
	<!ENTITY skos "http://www.w3.org/2004/02/skos/core#">
	<!ENTITY sm "http://www.omg.org/techprocess/ab/SpecificationMetadata/">
	<!ENTITY xsd "http://www.w3.org/2001/XMLSchema#">
]>
<rdf:RDF xml:base="https://tw.rpi.edu/ontology-engineering/oe2020/pokemon-moveset/"
	xmlns="https://tw.rpi.edu/ontology-engineering/oe2020/pokemon-moveset/"
	xmlns:dct="http://purl.org/dc/terms/"
	xmlns:fibo-fnd-aap-agt="https://spec.edmcouncil.org/fibo/ontology/FND/AgentsAndPeople/Agents/"
	xmlns:fibo-fnd-aap-ppl="https://spec.edmcouncil.org/fibo/ontology/FND/AgentsAndPeople/People/"
	xmlns:fibo-fnd-arr-cls="https://spec.edmcouncil.org/fibo/ontology/FND/Arrangements/ClassificationSchemes/"
	xmlns:fibo-fnd-arr-lif="https://spec.edmcouncil.org/fibo/ontology/FND/Arrangements/Lifecycles/"
	xmlns:fibo-fnd-dt-fd="https://spec.edmcouncil.org/fibo/ontology/FND/DatesAndTimes/FinancialDates/"
	xmlns:fibo-fnd-dt-oc="https://spec.edmcouncil.org/fibo/ontology/FND/DatesAndTimes/Occurrences/"
	xmlns:fibo-fnd-gao-obj="https://spec.edmcouncil.org/fibo/ontology/FND/GoalsAndObjectives/Objectives/"
	xmlns:fibo-fnd-org-fm="https://spec.edmcouncil.org/fibo/ontology/FND/Organizations/FormalOrganizations/"
	xmlns:fibo-fnd-plc-loc="https://spec.edmcouncil.org/fibo/ontology/FND/Places/Locations/"
	xmlns:fibo-fnd-pty-pty="https://spec.edmcouncil.org/fibo/ontology/FND/Parties/Parties/"
	xmlns:fibo-fnd-pty-rl="https://spec.edmcouncil.org/fibo/ontology/FND/Parties/Roles/"
	xmlns:fibo-fnd-qt-qtu="https://spec.edmcouncil.org/fibo/ontology/FND/Quantities/QuantitiesAndUnits/"
	xmlns:fibo-fnd-rel-rel="https://spec.edmcouncil.org/fibo/ontology/FND/Relations/Relations/"
	xmlns:fibo-fnd-utl-alx="https://spec.edmcouncil.org/fibo/ontology/FND/Utilities/Analytics/"
	xmlns:fibo-fnd-utl-av="https://spec.edmcouncil.org/fibo/ontology/FND/Utilities/AnnotationVocabulary/"
	xmlns:lcc-cr="https://www.omg.org/spec/LCC/Countries/CountryRepresentation/"
	xmlns:lcc-lr="https://www.omg.org/spec/LCC/Languages/LanguageRepresentation/"
	xmlns:oe2020-pkm-mvs="https://tw.rpi.edu/ontology-engineering/oe2020/pokemon-moveset/"
	xmlns:owl="http://www.w3.org/2002/07/owl#"
	xmlns:rdf="http://www.w3.org/1999/02/22-rdf-syntax-ns#"
	xmlns:rdfs="http://www.w3.org/2000/01/rdf-schema#"
	xmlns:skos="http://www.w3.org/2004/02/skos/core#"
	xmlns:sm="http://www.omg.org/techprocess/ab/SpecificationMetadata/"
	xmlns:xsd="http://www.w3.org/2001/XMLSchema#">
	
	<owl:Ontology rdf:about="https://tw.rpi.edu/ontology-engineering/oe2020/pokemon-moveset/">
		<rdfs:label>Pokemon Moveset Ontology</rdfs:label>
		<dct:abstract>This ontology ...</dct:abstract>
		<sm:dependsOn rdf:datatype="&xsd;anyURI">https://spec.edmcouncil.org/fibo/ontology/FND/</sm:dependsOn>
		<sm:dependsOn rdf:datatype="&xsd;anyURI">https://www.omg.org/spec/LCC/</sm:dependsOn>
		<owl:imports rdf:resource="https://spec.edmcouncil.org/fibo/ontology/FND/AgentsAndPeople/Agents/"/>
		<owl:imports rdf:resource="https://spec.edmcouncil.org/fibo/ontology/FND/AgentsAndPeople/People/"/>
		<owl:imports rdf:resource="https://spec.edmcouncil.org/fibo/ontology/FND/ClassificationSchemes/"/>
		<owl:imports rdf:resource="https://spec.edmcouncil.org/fibo/ontology/FND/DatesAndTimes/FinancialDates/"/>
		<owl:imports rdf:resource="https://spec.edmcouncil.org/fibo/ontology/FND/DatesAndTimes/Occurrences/"/>
		<owl:imports rdf:resource="https://spec.edmcouncil.org/fibo/ontology/FND/Lifecycles/"/>
		<owl:imports rdf:resource="https://spec.edmcouncil.org/fibo/ontology/FND/Organizations/FormalOrganizations/"/>
		<owl:imports rdf:resource="https://spec.edmcouncil.org/fibo/ontology/FND/Parties/Parties/"/>
		<owl:imports rdf:resource="https://spec.edmcouncil.org/fibo/ontology/FND/Parties/Roles/"/>
		<owl:imports rdf:resource="https://spec.edmcouncil.org/fibo/ontology/FND/Places/Locations/"/>
		<owl:imports rdf:resource="https://spec.edmcouncil.org/fibo/ontology/FND/Quantities/QuantitiesAndUnits/"/>
		<owl:imports rdf:resource="https://spec.edmcouncil.org/fibo/ontology/FND/Relations/Relations/"/>
		<owl:imports rdf:resource="https://spec.edmcouncil.org/fibo/ontology/FND/Utilities/Analytics/"/>
		<owl:imports rdf:resource="https://spec.edmcouncil.org/fibo/ontology/FND/Utilities/AnnotationVocabulary/"/>
		<owl:imports rdf:resource="https://spec.edmcouncil.org/fibo/ontology/GoalsAndObjectives/Objectives/"/>
		<owl:imports rdf:resource="https://www.omg.org/spec/LCC/Countries/CountryRepresentation/"/>
		<owl:imports rdf:resource="https://www.omg.org/spec/LCC/Languages/LanguageRepresentation/"/>
		<owl:versionIRI rdf:resource="https://tw.rpi.edu/ontology-engineering/oe2020/20201003/pokemon-moveset/"/>
	</owl:Ontology>
	
	<owl:Class rdf:about="&fibo-fnd-gao-obj;Strategy">
	</owl:Class>
	
	<owl:NamedIndividual rdf:about="&oe2020-pkm-mvs;AmorphousEggGroup">
		<rdf:type rdf:resource="&oe2020-pkm-mvs;EggGroup"/>
		<rdfs:label>Amorphous egg group</rdfs:label>
		<rdfs:comment>egg group consisting of Pokémon that are amorphous, having no definite form</rdfs:comment>
	</owl:NamedIndividual>
	
	<owl:NamedIndividual rdf:about="&oe2020-pkm-mvs;BugEggGroup">
		<rdf:type rdf:resource="&oe2020-pkm-mvs;EggGroup"/>
		<rdfs:label>Bug egg group</rdfs:label>
		<skos:definition>egg group consisting of Pokémon that are insectoid (bug-like) in appearance</skos:definition>
	</owl:NamedIndividual>
	
	<owl:Class rdf:about="&oe2020-pkm-mvs;Character">
		<rdfs:subClassOf rdf:resource="&fibo-fnd-aap-agt;AutonomousAgent"/>
		<rdfs:subClassOf>
			<owl:Restriction>
				<owl:onProperty rdf:resource="&lcc-lr;hasName"/>
				<owl:onDataRange rdf:resource="&xsd;string"/>
				<owl:qualifiedCardinality rdf:datatype="&xsd;nonNegativeInteger">1</owl:qualifiedCardinality>
			</owl:Restriction>
		</rdfs:subClassOf>
		<rdfs:label>character</rdfs:label>
		<skos:definition>animate figure within a creative work</skos:definition>
		<fibo-fnd-utl-av:adaptedFrom rdf:datatype="&xsd;anyURI">https://literarydevices.net/character/</fibo-fnd-utl-av:adaptedFrom>
	</owl:Class>
	
	<owl:NamedIndividual rdf:about="&oe2020-pkm-mvs;DittoEggGroup">
		<rdf:type rdf:resource="&oe2020-pkm-mvs;EggGroup"/>
		<rdfs:label>Ditto egg group</rdfs:label>
		<skos:definition>egg group consisting entirely of the Pokémon species &quot;Ditto&quot;</skos:definition>
	</owl:NamedIndividual>
	
	<owl:NamedIndividual rdf:about="&oe2020-pkm-mvs;DragonEggGroup">
		<rdf:type rdf:resource="&oe2020-pkm-mvs;EggGroup"/>
		<rdfs:label>Dragon egg group</rdfs:label>
		<skos:definition>egg group consisting of Pokémon that are draconic in appearance</skos:definition>
	</owl:NamedIndividual>
	
	<owl:Class rdf:about="&oe2020-pkm-mvs;EggGroup">
		<rdfs:subClassOf rdf:resource="&fibo-fnd-arr-cls;Classifier"/>
		<rdfs:subClassOf>
			<owl:Restriction>
				<owl:onProperty rdf:resource="&lcc-cr;classifies"/>
				<owl:someValuesFrom rdf:resource="&oe2020-pkm-mvs;Pokemon"/>
			</owl:Restriction>
		</rdfs:subClassOf>
		<rdfs:label>egg group</rdfs:label>
		<skos:definition>collection of Pokémon species that are able to interbreed</skos:definition>
	</owl:Class>
	
	<owl:Class rdf:about="&oe2020-pkm-mvs;EvolutionItem">
		<rdfs:subClassOf rdf:resource="&oe2020-pkm-mvs;Item"/>
		<rdfs:label>evolution item</rdfs:label>
		<skos:definition>item that causes a Pokémon to undergo evolution</skos:definition>
	</owl:Class>
	
	<owl:Class rdf:about="&oe2020-pkm-mvs;EvolutionMethod">
		<rdfs:subClassOf rdf:resource="&fibo-fnd-gao-obj;Strategy"/>
		<rdfs:label>evolution method</rdfs:label>
		<skos:definition>conditions for triggering evolution in a specific Pokémon</skos:definition>
	</owl:Class>
	
	<owl:Class rdf:about="&oe2020-pkm-mvs;EvolveByFriendship">
		<rdfs:subClassOf rdf:resource="&oe2020-pkm-mvs;EvolutionMethod"/>
		<rdfs:label>evolve by friendship</rdfs:label>
		<skos:definition>evolution method characterized by a required level of friendship with a Pokémon</skos:definition>
	</owl:Class>
	
	<owl:Class rdf:about="&oe2020-pkm-mvs;EvolveByItem">
		<rdfs:subClassOf rdf:resource="&oe2020-pkm-mvs;EvolutionMethod"/>
		<rdfs:label>evolve by item</rdfs:label>
		<skos:definition>evolution method characterized by the use of an item on a Pokémon</skos:definition>
	</owl:Class>
	
	<owl:Class rdf:about="&oe2020-pkm-mvs;EvolveByLevelUp">
		<rdfs:subClassOf rdf:resource="&oe2020-pkm-mvs;EvolutionMethod"/>
		<rdfs:label>evolve by level up</rdfs:label>
		<skos:definition>evolution method characterized by a minimum required Pokémon level</skos:definition>
	</owl:Class>
	
	<owl:Class rdf:about="&oe2020-pkm-mvs;EvolveByTimeOfDay">
		<rdfs:subClassOf rdf:resource="&oe2020-pkm-mvs;EvolutionMethod"/>
		<rdfs:label>evolve by time of day</rdfs:label>
		<skos:definition>evolution method characterized by a required time of day</skos:definition>
	</owl:Class>
	
	<owl:Class rdf:about="&oe2020-pkm-mvs;EvolveByTrade">
		<rdfs:subClassOf rdf:resource="&oe2020-pkm-mvs;EvolutionMethod"/>
		<rdfs:label>evolve by trade</rdfs:label>
		<skos:definition>evolution method characterized by a trade between two players</skos:definition>
	</owl:Class>
	
	<owl:Class rdf:about="&oe2020-pkm-mvs;EvolveByUniqueProcess">
		<rdfs:subClassOf rdf:resource="&oe2020-pkm-mvs;EvolutionMethod"/>
		<rdfs:label>evolve by unique process</rdfs:label>
		<skos:definition>evolution method characterized by a unique process or set of triggers</skos:definition>
	</owl:Class>
	
	<owl:NamedIndividual rdf:about="&oe2020-pkm-mvs;FairyEggGroup">
		<rdf:type rdf:resource="&oe2020-pkm-mvs;EggGroup"/>
		<rdfs:label>Fairy egg group</rdfs:label>
		<skos:definition>egg group consisting of Pokémon that are petite and considered very cute</skos:definition>
	</owl:NamedIndividual>
	
	<owl:NamedIndividual rdf:about="&oe2020-pkm-mvs;Female">
		<rdf:type rdf:resource="&oe2020-pkm-mvs;Gender"/>
		<rdfs:label>female</rdfs:label>
		<skos:definition>gender indicating that the Pokémon is female</skos:definition>
	</owl:NamedIndividual>
	
	<owl:NamedIndividual rdf:about="&oe2020-pkm-mvs;FieldEggGroup">
		<rdf:type rdf:resource="&oe2020-pkm-mvs;EggGroup"/>
		<rdfs:label>Field egg group</rdfs:label>
		<skos:definition>egg group consisting of Pokémon that are terrestrial in nature</skos:definition>
	</owl:NamedIndividual>
	
	<owl:NamedIndividual rdf:about="&oe2020-pkm-mvs;FlyingEggGroup">
		<rdf:type rdf:resource="&oe2020-pkm-mvs;EggGroup"/>
		<rdfs:label>Flying egg group</rdfs:label>
		<skos:definition>egg group consisting of Pokémon that are avian (bird-like) in appearance</skos:definition>
	</owl:NamedIndividual>
	
	<owl:Class rdf:about="&oe2020-pkm-mvs;Friendship">
		<rdfs:subClassOf rdf:resource="&oe2020-pkm-mvs;PokémonStatistic"/>
		<rdfs:label>friendship</rdfs:label>
		<owl:disjointWith rdf:resource="&oe2020-pkm-mvs;Level"/>
		<skos:definition>measure of a Pokémon&apos;s level of attachment to the player character</skos:definition>
	</owl:Class>
	
	<owl:Class rdf:about="&oe2020-pkm-mvs;Gender">
		<rdfs:subClassOf rdf:resource="&fibo-fnd-arr-cls;Classifier"/>
		<rdfs:subClassOf>
			<owl:Restriction>
				<owl:onProperty rdf:resource="&lcc-cr;classifies"/>
				<owl:someValuesFrom rdf:resource="&oe2020-pkm-mvs;Pokemon"/>
			</owl:Restriction>
		</rdfs:subClassOf>
		<rdfs:label>gender</rdfs:label>
		<skos:definition>classifier indicating a physical condition of a Pokémon with respect to breeding with other Pokémon</skos:definition>
		<fibo-fnd-utl-av:adaptedFrom rdf:datatype="&xsd;anyURI">https://www.dictionary.com/browse/gender</fibo-fnd-utl-av:adaptedFrom>
	</owl:Class>
	
	<owl:NamedIndividual rdf:about="&oe2020-pkm-mvs;GrassEggGroup">
		<rdf:type rdf:resource="&oe2020-pkm-mvs;EggGroup"/>
		<rdfs:label>Grass egg group</rdfs:label>
		<skos:definition>egg group consisting of Pokémon that are plant-like in appearance</skos:definition>
	</owl:NamedIndividual>
	
	<owl:NamedIndividual rdf:about="&oe2020-pkm-mvs;HumanLikeEggGroup">
		<rdf:type rdf:resource="&oe2020-pkm-mvs;EggGroup"/>
		<rdfs:label>Human-Like egg group</rdfs:label>
		<skos:definition>egg group consisting of Pokémon that are fully bipedal</skos:definition>
	</owl:NamedIndividual>
	
	<owl:Class rdf:about="&oe2020-pkm-mvs;Item">
		<rdfs:label>item</rdfs:label>
		<skos:definition>a in-game object that can be used on or by Pokémon</skos:definition>
	</owl:Class>
	
	<owl:Class rdf:about="&oe2020-pkm-mvs;LearnByInheritance">
		<rdfs:subClassOf rdf:resource="&oe2020-pkm-mvs;LearnMethod"/>
		<rdfs:label>learn by inheritance</rdfs:label>
		<skos:definition>learn method in which a move is learned by breeding two Pokémon</skos:definition>
	</owl:Class>
	
	<owl:Class rdf:about="&oe2020-pkm-mvs;LearnByItem">
		<rdfs:subClassOf rdf:resource="&oe2020-pkm-mvs;LearnMethod"/>
		<rdfs:label>learn by item</rdfs:label>
		<skos:definition>learn method in which a move is learned by using an item on a Pokémon</skos:definition>
	</owl:Class>
	
	<owl:Class rdf:about="&oe2020-pkm-mvs;LearnByLevelUp">
		<rdfs:subClassOf rdf:resource="&oe2020-pkm-mvs;LearnMethod"/>
		<rdfs:label>learn by level up</rdfs:label>
		<skos:definition>learn method in which a move is learned upon reaching a certain Pokémon level</skos:definition>
	</owl:Class>
	
	<owl:Class rdf:about="&oe2020-pkm-mvs;LearnByMoveTutor">
		<rdfs:subClassOf rdf:resource="&oe2020-pkm-mvs;LearnMethod"/>
		<rdfs:label>learn by move tutor</rdfs:label>
		<skos:definition>learn method in which a move is learned by interacting with a move tutor</skos:definition>
	</owl:Class>
	
	<owl:Class rdf:about="&oe2020-pkm-mvs;LearnMethod">
		<rdfs:subClassOf rdf:resource="&fibo-fnd-gao-obj;Strategy"/>
		<rdfs:label>learn method</rdfs:label>
		<skos:definition>conditions for acquiring a move</skos:definition>
	</owl:Class>
	
	<owl:Class rdf:about="&oe2020-pkm-mvs;Level">
		<rdfs:subClassOf rdf:resource="&oe2020-pkm-mvs;PokémonStatistic"/>
		<rdfs:label>level</rdfs:label>
		<skos:definition>measurement of Pokémon strength</skos:definition>
	</owl:Class>
	
	<owl:NamedIndividual rdf:about="&oe2020-pkm-mvs;Male">
		<rdf:type rdf:resource="&oe2020-pkm-mvs;Gender"/>
		<rdfs:label>male</rdfs:label>
		<skos:definition>gender indicating that the Pokémon is male</skos:definition>
	</owl:NamedIndividual>
	
	<owl:NamedIndividual rdf:about="&oe2020-pkm-mvs;MineralEggGroup">
		<rdf:type rdf:resource="&oe2020-pkm-mvs;EggGroup"/>
		<rdfs:label>Mineral egg group</rdfs:label>
		<skos:definition>egg group consisting of Pokémon that are inorganic in nature</skos:definition>
	</owl:NamedIndividual>
	
	<owl:NamedIndividual rdf:about="&oe2020-pkm-mvs;MonsterEggGroup">
		<rdf:type rdf:resource="&oe2020-pkm-mvs;EggGroup"/>
		<rdfs:label>Monster egg group</rdfs:label>
		<skos:definition>egg group consisting of Pokémon which are saurian in general</skos:definition>
	</owl:NamedIndividual>
	
	<owl:Class rdf:about="&oe2020-pkm-mvs;Move">
		<rdfs:label>move</rdfs:label>
		<skos:definition>ability or action a Pokémon can use</skos:definition>
	</owl:Class>
	
	<owl:Class rdf:about="&oe2020-pkm-mvs;MoveTutor">
		<rdfs:subClassOf rdf:resource="&oe2020-pkm-mvs;NonPlayerCharacter"/>
		<rdfs:label>move tutor</rdfs:label>
		<skos:definition>a non-player character who will teach a Pokémon specific moves</skos:definition>
	</owl:Class>
	
	<owl:NamedIndividual rdf:about="&oe2020-pkm-mvs;NonBinary">
		<rdf:type rdf:resource="&oe2020-pkm-mvs;Gender"/>
		<rdfs:label>non-binary</rdfs:label>
		<rdfs:comment>for use with the Pokémon Ditto</rdfs:comment>
		<skos:definition>gender indicating that the Pokémon is not exclusively masculine or feminine, i.e., it can breed with any other Pokémon with respect to gender</skos:definition>
	</owl:NamedIndividual>
	
	<owl:Class rdf:about="&oe2020-pkm-mvs;NonPlayerCharacter">
		<rdfs:subClassOf rdf:resource="&oe2020-pkm-mvs;Character"/>
		<rdfs:label>non-player character</rdfs:label>
		<owl:disjointWith rdf:resource="&oe2020-pkm-mvs;PlayerCharacter"/>
		<skos:definition>character whose actions cannot be controlled by the player (i.e., person operating the handheld or console)</skos:definition>
		<fibo-fnd-utl-av:abbreviation>NPC</fibo-fnd-utl-av:abbreviation>
		<fibo-fnd-utl-av:adaptedFrom rdf:datatype="&xsd;anyURI">https://bulbapedia.bulbagarden.net/wiki/Non-player_character</fibo-fnd-utl-av:adaptedFrom>
	</owl:Class>
	
	<owl:Class rdf:about="&oe2020-pkm-mvs;ObtainFromBreeding">
		<rdfs:subClassOf rdf:resource="&oe2020-pkm-mvs;ObtainMethod"/>
		<rdfs:label>obtain from breeding</rdfs:label>
		<skos:definition>obtain method characterized by a Pokémon species being obtainable exclusively by breeding two Pokémon</skos:definition>
	</owl:Class>
	
	<owl:Class rdf:about="&oe2020-pkm-mvs;ObtainFromEgg">
		<rdfs:subClassOf rdf:resource="&oe2020-pkm-mvs;ObtainMethod"/>
		<rdfs:label>obtain from egg</rdfs:label>
		<skos:definition>obtain method characterized by a Pokémon species being obtainable exclusively through hatching an egg that is received from in-game (via story progression or some non-player character)</skos:definition>
	</owl:Class>
	
	<owl:Class rdf:about="&oe2020-pkm-mvs;ObtainFromEvent">
		<rdfs:subClassOf rdf:resource="&oe2020-pkm-mvs;ObtainMethod"/>
		<rdfs:label>obtain from event</rdfs:label>
		<skos:definition>obtain method characterized by a Pokémon species being obtainable exclusively through a Pokémon event</skos:definition>
	</owl:Class>
	
	<owl:Class rdf:about="&oe2020-pkm-mvs;ObtainFromNPC">
		<rdfs:subClassOf rdf:resource="&oe2020-pkm-mvs;ObtainMethod"/>
		<rdfs:label>obtain from non-player character</rdfs:label>
		<skos:definition>obtain method characterized by a Pokémon species being obtainable exclusively through interaction with a non-player character</skos:definition>
	</owl:Class>
	
	<owl:Class rdf:about="&oe2020-pkm-mvs;ObtainFromTrade">
		<rdfs:subClassOf rdf:resource="&oe2020-pkm-mvs;ObtainMethod"/>
		<rdfs:label>obtain from trade</rdfs:label>
		<skos:definition>obtain method characterized by a Pokémon species being obtainable exclusively via trading with between two players</skos:definition>
	</owl:Class>
	
	<owl:Class rdf:about="&oe2020-pkm-mvs;ObtainFromWild">
		<rdfs:subClassOf rdf:resource="&oe2020-pkm-mvs;ObtainMethod"/>
		<rdfs:label>obtain from wild</rdfs:label>
		<skos:definition>obtain method characterized by a Pokémon species being obtainable through wild encounters in a specific Pokémon location</skos:definition>
	</owl:Class>
	
	<owl:Class rdf:about="&oe2020-pkm-mvs;ObtainMethod">
		<rdfs:subClassOf rdf:resource="&fibo-fnd-gao-obj;Strategy"/>
		<rdfs:label>obtain method</rdfs:label>
		<skos:definition>strategy employed by a player for adding a Pokémon to their collection</skos:definition>
	</owl:Class>
	
	<owl:Class rdf:about="&oe2020-pkm-mvs;Player">
		<rdfs:subClassOf rdf:resource="&fibo-fnd-pty-pty;PartyInRole"/>
		<rdfs:subClassOf>
			<owl:Restriction>
				<owl:onProperty rdf:resource="&fibo-fnd-rel-rel;hasIdentity"/>
				<owl:onClass rdf:resource="&fibo-fnd-aap-ppl;Person"/>
				<owl:qualifiedCardinality rdf:datatype="&xsd;nonNegativeInteger">1</owl:qualifiedCardinality>
			</owl:Restriction>
		</rdfs:subClassOf>
		<rdfs:label>player</rdfs:label>
		<skos:definition>person who takes part or is skilled in Pokémon games</skos:definition>
		<fibo-fnd-utl-av:adaptedFrom rdf:datatype="&xsd;anyURI">https://www.collinsdictionary.com/dictionary/english/player</fibo-fnd-utl-av:adaptedFrom>
	</owl:Class>
	
	<owl:Class rdf:about="&oe2020-pkm-mvs;PlayerCharacter">
		<rdfs:subClassOf rdf:resource="&oe2020-pkm-mvs;Character"/>
		<rdfs:subClassOf>
			<owl:Restriction>
				<owl:onProperty rdf:resource="&fibo-fnd-rel-rel;represents"/>
				<owl:onClass rdf:resource="&oe2020-pkm-mvs;Player"/>
				<owl:qualifiedCardinality rdf:datatype="&xsd;nonNegativeInteger">1</owl:qualifiedCardinality>
			</owl:Restriction>
		</rdfs:subClassOf>
		<rdfs:label>player character</rdfs:label>
		<skos:definition>main character in a Pokémon game that is an avatar for a human player</skos:definition>
		<fibo-fnd-utl-av:adaptedFrom rdf:datatype="&xsd;anyURI">https://bulbapedia.bulbagarden.net/wiki/Player_character</fibo-fnd-utl-av:adaptedFrom>
		<fibo-fnd-utl-av:explanatoryNote>It is left up to the real player to &apos;fill in&apos; what they imagine the character is feeling, thinking, and acting, thus immersing them within the world of the game.</fibo-fnd-utl-av:explanatoryNote>
	</owl:Class>
	
	<owl:Class rdf:about="&oe2020-pkm-mvs;Pokemon">
		<rdfs:subClassOf rdf:resource="&oe2020-pkm-mvs;Character"/>
		<rdfs:subClassOf>
			<owl:Restriction>
				<owl:onProperty rdf:resource="&oe2020-pkm-mvs;hasGender"/>
				<owl:someValuesFrom rdf:resource="&oe2020-pkm-mvs;Gender"/>
			</owl:Restriction>
		</rdfs:subClassOf>
		<rdfs:label>Pokémon</rdfs:label>
		<skos:definition>fictional, animated monster that can be captured by a player and trained to fight with other monsters on behalf of the player</skos:definition>
	</owl:Class>
	
	<owl:Class rdf:about="&oe2020-pkm-mvs;PokemonFamily">
		<rdfs:subClassOf rdf:resource="&fibo-fnd-org-fm;Group"/>
		<rdfs:subClassOf>
			<owl:Restriction>
				<owl:onProperty rdf:resource="&lcc-lr;hasMember"/>
				<owl:someValuesFrom rdf:resource="&oe2020-pkm-mvs;Pokemon"/>
			</owl:Restriction>
		</rdfs:subClassOf>
		<rdfs:label>Pokémon family</rdfs:label>
		<skos:definition>set of Pokémon related by evolution</skos:definition>
		<fibo-fnd-utl-av:explanatoryNote>The species at the lowest evolutionary stage in an evolutionary family can ultimately evolve into any member of the evolutionary family.</fibo-fnd-utl-av:explanatoryNote>
	</owl:Class>
	
	<owl:Class rdf:about="&oe2020-pkm-mvs;PokémonEgg">
		<rdfs:subClassOf rdf:resource="&oe2020-pkm-mvs;Pokemon"/>
		<rdfs:label>Pokémon egg</rdfs:label>
		<skos:definition>result of breeding two Pokémon together</skos:definition>
	</owl:Class>
	
	<owl:Class rdf:about="&oe2020-pkm-mvs;PokémonEvent">
		<rdfs:subClassOf rdf:resource="&fibo-fnd-dt-oc;Occurrence"/>
		<rdfs:label>Pokémon event</rdfs:label>
		<skos:definition>a promotional event in which a Pokémon is distributed</skos:definition>
	</owl:Class>
	
	<owl:Class rdf:about="&oe2020-pkm-mvs;PokémonLocation">
		<rdfs:subClassOf rdf:resource="&lcc-cr;Location"/>
		<rdfs:subClassOf>
			<owl:Restriction>
				<owl:onProperty rdf:resource="&lcc-lr;hasName"/>
				<owl:onDataRange rdf:resource="&xsd;string"/>
				<owl:qualifiedCardinality rdf:datatype="&xsd;nonNegativeInteger">1</owl:qualifiedCardinality>
			</owl:Restriction>
		</rdfs:subClassOf>
		<rdfs:label>Pokémon location</rdfs:label>
		<skos:definition>a location in a Pokémon game</skos:definition>
	</owl:Class>
	
	<owl:Class rdf:about="&oe2020-pkm-mvs;PokémonStatistic">
		<rdfs:subClassOf rdf:resource="&fibo-fnd-qt-qtu;QuantityValue"/>
		<rdfs:subClassOf rdf:resource="&fibo-fnd-utl-alx;Aspect"/>
		<rdfs:label>Pokémon statistic</rdfs:label>
		<skos:definition>value or measure associated with some Pokémon</skos:definition>
	</owl:Class>
	
	<owl:Class rdf:about="&oe2020-pkm-mvs;TechnicalMachine">
		<rdfs:subClassOf rdf:resource="&oe2020-pkm-mvs;Item"/>
		<rdfs:label>technical machine</rdfs:label>
		<skos:definition>item that can be used to teach a Pokémon a move (infinite uses)</skos:definition>
	</owl:Class>
	
	<owl:Class rdf:about="&oe2020-pkm-mvs;TechnicalRecord">
		<rdfs:subClassOf rdf:resource="&oe2020-pkm-mvs;Item"/>
		<rdfs:label>technical record</rdfs:label>
		<skos:definition>item that can be used to teach a Pokémon a move (single uses)</skos:definition>
	</owl:Class>
	
	<owl:NamedIndividual rdf:about="&oe2020-pkm-mvs;UndiscoveredEggGroup">
		<rdf:type rdf:resource="&oe2020-pkm-mvs;EggGroup"/>
		<rdfs:label>Undiscovered egg group</rdfs:label>
	</owl:NamedIndividual>
	
	<owl:NamedIndividual rdf:about="&oe2020-pkm-mvs;UnknownGender">
		<rdf:type rdf:resource="&oe2020-pkm-mvs;Gender"/>
		<rdfs:label>non-binary</rdfs:label>
		<rdfs:comment>for use with unknown gendered Pokémon, excluding the Pokémon Ditto</rdfs:comment>
		<skos:definition>gender indicating that the nature of the Pokémon&apos;s sexuality is not known</skos:definition>
	</owl:NamedIndividual>
	
	<owl:NamedIndividual rdf:about="&oe2020-pkm-mvs;Water1EggGroup">
		<rdf:type rdf:resource="&oe2020-pkm-mvs;EggGroup"/>
		<rdfs:label>Water 1 egg group</rdfs:label>
		<skos:definition>egg group consisting of Pokémon that are amphibious in nature</skos:definition>
	</owl:NamedIndividual>
	
	<owl:NamedIndividual rdf:about="&oe2020-pkm-mvs;Water2EggGroup">
		<rdf:type rdf:resource="&oe2020-pkm-mvs;EggGroup"/>
		<rdfs:label>Water 2 egg group</rdfs:label>
		<skos:definition>egg group consisting of Pokémon that are piscine (fish-like) in appearance</skos:definition>
	</owl:NamedIndividual>
	
	<owl:NamedIndividual rdf:about="&oe2020-pkm-mvs;Water3EggGroup">
		<rdf:type rdf:resource="&oe2020-pkm-mvs;EggGroup"/>
		<rdfs:label>Water 3 egg group</rdfs:label>
		<skos:definition>egg group consisting of Pokémon that resemble aquatic invertebrates</skos:definition>
	</owl:NamedIndividual>
	
	<owl:ObjectProperty rdf:about="&oe2020-pkm-mvs;fromEvent">
		<rdfs:label>from event</rdfs:label>
		<skos:definition>indicates a specific Pokémon event in which a specific Pokémon or item is distributed</skos:definition>
	</owl:ObjectProperty>
	
	<owl:ObjectProperty rdf:about="&oe2020-pkm-mvs;fromItem">
		<rdfs:label>from item</rdfs:label>
		<skos:definition>indicates a move can be learned from a specific item</skos:definition>
	</owl:ObjectProperty>
	
	<owl:ObjectProperty rdf:about="&oe2020-pkm-mvs;fromNonPlayerCharacter">
		<rdfs:label>from non-player character</rdfs:label>
		<skos:definition>indicates that a Pokémon egg, item, or move can be obtained from a non-player character</skos:definition>
	</owl:ObjectProperty>
	
	<owl:ObjectProperty rdf:about="&oe2020-pkm-mvs;fromParent">
		<rdfs:label>from parent</rdfs:label>
		<skos:definition>indicates a move can be inherited from a specific Pokémon</skos:definition>
	</owl:ObjectProperty>
	
	<owl:ObjectProperty rdf:about="&oe2020-pkm-mvs;hasAssociatedMove">
		<rdfs:label>has associated move</rdfs:label>
		<skos:definition>indicates a specific move is associated with a learn method</skos:definition>
	</owl:ObjectProperty>
	
	<owl:ObjectProperty rdf:about="&oe2020-pkm-mvs;hasEggGroup">
		<rdfs:subPropertyOf rdf:resource="&lcc-cr;isClassifiedBy"/>
		<rdfs:label>has egg group</rdfs:label>
		<rdfs:domain rdf:resource="&oe2020-pkm-mvs;Pokemon"/>
		<rdfs:range rdf:resource="&oe2020-pkm-mvs;EggGroup"/>
		<skos:definition>indicates the group of Pokémon with which a Pokémon is able to breed successfully</skos:definition>
	</owl:ObjectProperty>
	
	<owl:ObjectProperty rdf:about="&oe2020-pkm-mvs;hasEvolutionMethod">
		<rdfs:subPropertyOf rdf:resource="&oe2020-pkm-mvs;hasStrategy"/>
		<rdfs:label>has evolution method</rdfs:label>
		<skos:definition>indicates the method by which a Pokémon evolves</skos:definition>
	</owl:ObjectProperty>
	
	<owl:ObjectProperty rdf:about="&oe2020-pkm-mvs;hasFriendship">
		<rdfs:subPropertyOf rdf:resource="&oe2020-pkm-mvs;hasPokémonStatistic"/>
		<rdfs:label>has friendship</rdfs:label>
		<skos:definition>indicates a specific Pokémon has a specific friendship level or must have a specific friendship level for an event to occur</skos:definition>
	</owl:ObjectProperty>
	
	<owl:ObjectProperty rdf:about="&oe2020-pkm-mvs;hasGender">
		<rdfs:subPropertyOf rdf:resource="&lcc-cr;isClassifiedBy"/>
		<rdfs:label>has gender</rdfs:label>
		<rdfs:range rdf:resource="&oe2020-pkm-mvs;Gender"/>
		<skos:definition>indicates the physical condition of a Pokémon with respect to sexuality</skos:definition>
	</owl:ObjectProperty>
	
	<owl:ObjectProperty rdf:about="&oe2020-pkm-mvs;hasLearnMethod">
		<rdfs:subPropertyOf rdf:resource="&oe2020-pkm-mvs;hasStrategy"/>
		<rdfs:label>has learn method</rdfs:label>
		<skos:definition>indicates the method by which a Pokémon can learn a move</skos:definition>
	</owl:ObjectProperty>
	
	<owl:ObjectProperty rdf:about="&oe2020-pkm-mvs;hasLevel">
		<rdfs:subPropertyOf rdf:resource="&oe2020-pkm-mvs;hasPokémonStatistic"/>
		<rdfs:label>has level</rdfs:label>
		<skos:definition>indicates a specific Pokémon has a specific level or must have a specific level for an event to occur</skos:definition>
	</owl:ObjectProperty>
	
	<owl:ObjectProperty rdf:about="&oe2020-pkm-mvs;hasObtainMethod">
		<rdfs:subPropertyOf rdf:resource="&oe2020-pkm-mvs;hasStrategy"/>
		<rdfs:label>has obtain method</rdfs:label>
		<skos:definition>indicates the method by which a Pokémon can be obtained</skos:definition>
	</owl:ObjectProperty>
	
	<owl:ObjectProperty rdf:about="&oe2020-pkm-mvs;hasPokémonStatistic">
		<rdfs:label>has Pokémon statistic</rdfs:label>
		<skos:definition>indicates that a Pokémon has a Pokémon statistic or must have a some value for an event to occur</skos:definition>
	</owl:ObjectProperty>
	
	<owl:ObjectProperty rdf:about="&oe2020-pkm-mvs;hasStrategy">
		<rdfs:label>has strategy</rdfs:label>
		<skos:definition>indicates relation to a specific strategy</skos:definition>
	</owl:ObjectProperty>
	
	<owl:ObjectProperty rdf:about="&oe2020-pkm-mvs;precedes">
		<rdfs:subPropertyOf rdf:resource="&oe2020-pkm-mvs;relatesTo"/>
		<rdfs:label>precedes</rdfs:label>
		<owl:inverseOf rdf:resource="&oe2020-pkm-mvs;succeeds"/>
		<skos:definition>relates a stage in a lifecycle, an event, or occurrence, such as a breeding event, to one that occurs before it</skos:definition>
		<fibo-fnd-utl-av:adaptedFrom rdf:datatype="&xsd;anyURI">https://www.merriam-webster.com/dictionary/precede</fibo-fnd-utl-av:adaptedFrom>
	</owl:ObjectProperty>
	
	<owl:ObjectProperty rdf:about="&oe2020-pkm-mvs;relatesTo">
		<rdfs:label>relates to</rdfs:label>
		<skos:definition>has a logical or causal connection with</skos:definition>
		<fibo-fnd-utl-av:adaptedFrom rdf:datatype="&xsd;anyURI">https://www.merriam-webster.com/dictionary/relates</fibo-fnd-utl-av:adaptedFrom>
	</owl:ObjectProperty>
	
	<owl:ObjectProperty rdf:about="&oe2020-pkm-mvs;succeeds">
		<rdfs:subPropertyOf rdf:resource="&oe2020-pkm-mvs;relatesTo"/>
		<rdfs:label>succeeds</rdfs:label>
		<skos:definition>relates a stage in a lifecycle, an event, or occurrence, such as a breeding event, to one that follows it</skos:definition>
		<fibo-fnd-utl-av:adaptedFrom rdf:datatype="&xsd;anyURI">https://www.merriam-webster.com/dictionary/succeed</fibo-fnd-utl-av:adaptedFrom>
	</owl:ObjectProperty>
	
	<owl:ObjectProperty rdf:about="&oe2020-pkm-mvs;teachesMove">
		<rdfs:label>teaches move</rdfs:label>
		<skos:definition>indicates that an item or non-player character is able to teach a Pokémon a specific move</skos:definition>
	</owl:ObjectProperty>
	
	<owl:AllDisjointClasses>
		<owl:members rdf:parseType="Collection">
			<rdf:Description rdf:about="&oe2020-pkm-mvs;EvolutionItem">
			</rdf:Description>
			<rdf:Description rdf:about="&oe2020-pkm-mvs;TechnicalMachine">
			</rdf:Description>
			<rdf:Description rdf:about="&oe2020-pkm-mvs;TechnicalRecord">
			</rdf:Description>
		</owl:members>
	</owl:AllDisjointClasses>
	<owl:AllDisjointClasses>
		<owl:members rdf:parseType="Collection">
			<rdf:Description rdf:about="&oe2020-pkm-mvs;EvolveByFriendship">
			</rdf:Description>
			<rdf:Description rdf:about="&oe2020-pkm-mvs;EvolveByItem">
			</rdf:Description>
			<rdf:Description rdf:about="&oe2020-pkm-mvs;EvolveByLevelUp">
			</rdf:Description>
			<rdf:Description rdf:about="&oe2020-pkm-mvs;EvolveByTimeOfDay">
			</rdf:Description>
			<rdf:Description rdf:about="&oe2020-pkm-mvs;EvolveByTrade">
			</rdf:Description>
			<rdf:Description rdf:about="&oe2020-pkm-mvs;EvolveByUniqueProcess">
			</rdf:Description>
		</owl:members>
	</owl:AllDisjointClasses>
	<owl:AllDisjointClasses>
		<owl:members rdf:parseType="Collection">
			<rdf:Description rdf:about="&oe2020-pkm-mvs;LearnByInheritance">
			</rdf:Description>
			<rdf:Description rdf:about="&oe2020-pkm-mvs;LearnByItem">
			</rdf:Description>
			<rdf:Description rdf:about="&oe2020-pkm-mvs;LearnByLevelUp">
			</rdf:Description>
			<rdf:Description rdf:about="&oe2020-pkm-mvs;LearnByMoveTutor">
			</rdf:Description>
		</owl:members>
	</owl:AllDisjointClasses>
	<owl:AllDisjointClasses>
		<owl:members rdf:parseType="Collection">
			<rdf:Description rdf:about="&oe2020-pkm-mvs;ObtainFromBreeding">
			</rdf:Description>
			<rdf:Description rdf:about="&oe2020-pkm-mvs;ObtainFromEgg">
			</rdf:Description>
			<rdf:Description rdf:about="&oe2020-pkm-mvs;ObtainFromEvent">
			</rdf:Description>
			<rdf:Description rdf:about="&oe2020-pkm-mvs;ObtainFromNPC">
			</rdf:Description>
			<rdf:Description rdf:about="&oe2020-pkm-mvs;ObtainFromTrade">
			</rdf:Description>
			<rdf:Description rdf:about="&oe2020-pkm-mvs;ObtainFromWild">
			</rdf:Description>
		</owl:members>
	</owl:AllDisjointClasses>
</rdf:RDF>