<?xml version="1.0" encoding="UTF-8"?>
<!DOCTYPE rdf:RDF [
	<!ENTITY cmns-av "https://www.omg.org/spec/Commons/AnnotationVocabulary/">
	<!ENTITY cmns-doc "https://www.omg.org/spec/Commons/Documents/">
	<!ENTITY cmns-dt "https://www.omg.org/spec/Commons/DatesAndTimes/">
	<!ENTITY cmns-org "https://www.omg.org/spec/Commons/Organizations/">
	<!ENTITY cmns-pts "https://www.omg.org/spec/Commons/PartiesAndSituations/">
	<!ENTITY cmns-rlcmp "https://www.omg.org/spec/Commons/RolesAndCompositions/">
	<!ENTITY dct "http://purl.org/dc/terms/">
	<!ENTITY oe-wtgw "https://tw.rpi.edu/ontology-engineering/oe2024/when-to-go-where/WhenToGoWhere/">
	<!ENTITY owl "http://www.w3.org/2002/07/owl#">
	<!ENTITY rdf "http://www.w3.org/1999/02/22-rdf-syntax-ns#">
	<!ENTITY rdfs "http://www.w3.org/2000/01/rdf-schema#">
	<!ENTITY skos "http://www.w3.org/2004/02/skos/core#">
	<!ENTITY xsd "http://www.w3.org/2001/XMLSchema#">
]>
<rdf:RDF xml:base="https://tw.rpi.edu/ontology-engineering/oe2024/when-to-go-where/WhenToGoWhere/"
	xmlns="https://tw.rpi.edu/ontology-engineering/oe2024/when-to-go-where/WhenToGoWhere/"
	xmlns:cmns-av="https://www.omg.org/spec/Commons/AnnotationVocabulary/"
	xmlns:cmns-doc="https://www.omg.org/spec/Commons/Documents/"
	xmlns:cmns-dt="https://www.omg.org/spec/Commons/DatesAndTimes/"
	xmlns:cmns-org="https://www.omg.org/spec/Commons/Organizations/"
	xmlns:cmns-pts="https://www.omg.org/spec/Commons/PartiesAndSituations/"
	xmlns:cmns-rlcmp="https://www.omg.org/spec/Commons/RolesAndCompositions/"
	xmlns:dct="http://purl.org/dc/terms/"
	xmlns:oe-wtgw="https://tw.rpi.edu/ontology-engineering/oe2024/when-to-go-where/WhenToGoWhere/"
	xmlns:owl="http://www.w3.org/2002/07/owl#"
	xmlns:rdf="http://www.w3.org/1999/02/22-rdf-syntax-ns#"
	xmlns:rdfs="http://www.w3.org/2000/01/rdf-schema#"
	xmlns:skos="http://www.w3.org/2004/02/skos/core#"
	xmlns:xsd="http://www.w3.org/2001/XMLSchema#">
	
	<owl:Ontology rdf:about="https://tw.rpi.edu/ontology-engineering/oe2024/when-to-go-where/WhenToGoWhere/">
		<dct:abstract>some description</dct:abstract>
		<dct:creator>Annabelle Choi</dct:creator>
		<dct:creator>Ben Rodgers</dct:creator>
		<dct:creator>Samyuth Sagi</dct:creator>
		<dct:creator>Tyler Layton</dct:creator>
		<dct:license rdf:datatype="&xsd;anyURI">https://opensource.org/licenses/MIT</dct:license>
		<owl:imports rdf:resource="https://www.omg.org/spec/Commons/AnnotationVocabulary/"/>
		<owl:imports rdf:resource="https://www.omg.org/spec/Commons/DatesAndTimes/"/>
		<owl:imports rdf:resource="https://www.omg.org/spec/Commons/Documents/"/>
		<owl:imports rdf:resource="https://www.omg.org/spec/Commons/Organizations/"/>
		<owl:imports rdf:resource="https://www.omg.org/spec/Commons/PartiesAndSituations/"/>
		<owl:imports rdf:resource="https://www.omg.org/spec/Commons/RolesAndCompositions/"/>
	</owl:Ontology>
	
	<owl:Class rdf:about="&oe-wtgw;Accomodation">
		<rdfs:label>accomodation</rdfs:label>
		<skos:definition>temporary lodgings, sometimes also including board</skos:definition>
	</owl:Class>
	
	<owl:Class rdf:about="&oe-wtgw;Activity">
		<rdfs:label>activity</rdfs:label>
		<skos:definition>a use of the park by visitors</skos:definition>
	</owl:Class>
	
	<owl:Class rdf:about="&oe-wtgw;Amphibian">
		<rdfs:subClassOf rdf:resource="&oe-wtgw;Animal"/>
		<rdfs:label>amphibian</rdfs:label>
		<skos:definition>a cold-blooded vertebrate animal that typically starts life in water with gills and later develops lungs for life on land, such as frogs and salamanders</skos:definition>
	</owl:Class>
	
	<owl:Class rdf:about="&oe-wtgw;Amphitheatre">
		<rdfs:subClassOf rdf:resource="&oe-wtgw;Facility"/>
		<rdfs:label>amphitheatre</rdfs:label>
		<skos:definition>a circular or oval open-air venue with seating around a central performance area, often used for events in parks or natural settings</skos:definition>
	</owl:Class>
	
	<owl:Class rdf:about="&oe-wtgw;Animal">
		<rdfs:subClassOf>
			<owl:Restriction>
				<owl:onProperty rdf:resource="&oe-wtgw;hasDietaryPattern"/>
				<owl:someValuesFrom rdf:resource="&oe-wtgw;DietaryPattern"/>
			</owl:Restriction>
		</rdfs:subClassOf>
		<rdfs:subClassOf>
			<owl:Restriction>
				<owl:onProperty rdf:resource="&oe-wtgw;hasHabit"/>
				<owl:someValuesFrom rdf:resource="&oe-wtgw;Habit"/>
			</owl:Restriction>
		</rdfs:subClassOf>
		<rdfs:label>animal</rdfs:label>
		<skos:definition>a living organism that feeds on organic matter, typically having specialized sense organs and nervous systems and able to move voluntarily</skos:definition>
	</owl:Class>
	
	<owl:Class rdf:about="&oe-wtgw;AutoCaravan">
		<rdfs:subClassOf rdf:resource="&oe-wtgw;Activity"/>
		<rdfs:label>auto caravan</rdfs:label>
		<skos:definition>a motor vehicle equipped for living in, typically used for recreational purposes, often referred to as a camper van or motorhome.</skos:definition>
	</owl:Class>
	
	<owl:Class rdf:about="&oe-wtgw;AvgSeasonalTemperature">
		<rdfs:subClassOf rdf:resource="&oe-wtgw;AvgTemperature"/>
		<rdfs:subClassOf>
			<owl:Restriction>
				<owl:onProperty rdf:resource="&oe-wtgw;temperatureHasSeason"/>
				<owl:someValuesFrom rdf:resource="&oe-wtgw;Season"/>
			</owl:Restriction>
		</rdfs:subClassOf>
		<rdfs:label>average seasonal temperature</rdfs:label>
		<skos:definition>the mean thermal reading of a specific place over a part of the year</skos:definition>
	</owl:Class>
	
	<owl:Class rdf:about="&oe-wtgw;AvgTemperature">
		<rdfs:subClassOf>
			<owl:Restriction>
				<owl:onProperty rdf:resource="&oe-wtgw;hasTemperature"/>
				<owl:someValuesFrom rdf:resource="&xsd;decimal"/>
			</owl:Restriction>
		</rdfs:subClassOf>
		<rdfs:label>average temperature</rdfs:label>
		<skos:definition>the mean thermal reading of a specific place</skos:definition>
	</owl:Class>
	
	<owl:Class rdf:about="&oe-wtgw;BaldEagle">
		<rdfs:subClassOf rdf:resource="&oe-wtgw;Bird"/>
		<rdfs:label>bald eagle</rdfs:label>
		<skos:definition>subclass of the Bird Class that describes a Bald Eagle</skos:definition>
	</owl:Class>
	
	<owl:Class rdf:about="&oe-wtgw;Bird">
		<rdfs:subClassOf rdf:resource="&oe-wtgw;Animal"/>
		<rdfs:label>bird</rdfs:label>
		<skos:definition>a warm-blooded vertebrate animal characterized by feathers, beaks, and typically the ability to fly, with most species laying eggs</skos:definition>
	</owl:Class>
	
	<owl:Class rdf:about="&oe-wtgw;BlackBear">
		<rdfs:subClassOf rdf:resource="&oe-wtgw;Mammal"/>
		<rdfs:label>black bear</rdfs:label>
		<skos:definition>subclass of Mammal Class that describes a Black Bear</skos:definition>
	</owl:Class>
	
	<owl:Class rdf:about="&oe-wtgw;CampGround">
		<rdfs:subClassOf rdf:resource="&oe-wtgw;Accomodation"/>
		<rdfs:label>camp ground</rdfs:label>
		<skos:definition>a designated area in parks or recreational areas where visitors can set up tents or park recreational vehicles for overnight stays</skos:definition>
	</owl:Class>
	
	<owl:Class rdf:about="&oe-wtgw;Caribou">
		<rdfs:subClassOf rdf:resource="&oe-wtgw;Mammal"/>
		<rdfs:label>caribou</rdfs:label>
		<skos:definition>subclass of Mammal Class that describes a Caribou</skos:definition>
	</owl:Class>
	
	<owl:Class rdf:about="&oe-wtgw;Carnivore">
		<rdfs:subClassOf rdf:resource="&oe-wtgw;DietaryPattern"/>
		<rdfs:label>carnivore</rdfs:label>
		<owl:disjointWith rdf:resource="&oe-wtgw;Herbivore"/>
		<owl:disjointWith rdf:resource="&oe-wtgw;Omnivore"/>
		<skos:definition>an animal that primarily eats other animals, or meat</skos:definition>
	</owl:Class>
	
	<owl:Class rdf:about="&oe-wtgw;Climate">
		<rdfs:label>climate</rdfs:label>
		<skos:definition>the average weather conditions in a particular region over a long period, including temperature, humidity, wind patterns, and precipitation</skos:definition>
	</owl:Class>
	
	<owl:Class rdf:about="&oe-wtgw;Cold">
		<rdfs:subClassOf rdf:resource="&oe-wtgw;Climate"/>
		<rdfs:label>cold</rdfs:label>
		<skos:definition>having or being a temperature that is uncomfortably low for humans</skos:definition>
	</owl:Class>
	
	<owl:Class rdf:about="&oe-wtgw;ComfortStation">
		<rdfs:subClassOf rdf:resource="&oe-wtgw;Facility"/>
		<rdfs:label>comfort station</rdfs:label>
		<skos:definition>a facility with restrooms, sinks, and sometimes showers, provided for public use, especially in camping or recreational areas</skos:definition>
	</owl:Class>
	
	<owl:Class rdf:about="&oe-wtgw;Coyote">
		<rdfs:subClassOf rdf:resource="&oe-wtgw;Mammal"/>
		<rdfs:label>coyote</rdfs:label>
		<skos:definition>subclass of Mammal Class that describes a Coyote</skos:definition>
	</owl:Class>
	
	<owl:Class rdf:about="&oe-wtgw;DietaryPattern">
		<rdfs:label>dietary pattern</rdfs:label>
		<skos:definition>the habitual eating behaviors and food choices of an individual or group, often categorized by food type, frequency, and portion size</skos:definition>
	</owl:Class>
	
	<owl:Class rdf:about="&oe-wtgw;Difficulty">
		<rdfs:label>difficulty</rdfs:label>
		<skos:definition>A rating assigned by the National Park Service that lets visitors know how intensive a particular trail is</skos:definition>
	</owl:Class>
	
	<owl:Class rdf:about="&oe-wtgw;Dryland">
		<rdfs:subClassOf rdf:resource="&oe-wtgw;Terrain"/>
		<rdfs:subClassOf>
			<owl:Restriction>
				<owl:onProperty rdf:resource="&oe-wtgw;hasClimate"/>
				<owl:someValuesFrom>
					<owl:Class>
						<owl:unionOf rdf:parseType="Collection">
							<rdf:Description rdf:about="&oe-wtgw;Sunny">
							</rdf:Description>
							<rdf:Description rdf:about="&oe-wtgw;Windy">
							</rdf:Description>
						</owl:unionOf>
					</owl:Class>
				</owl:someValuesFrom>
			</owl:Restriction>
		</rdfs:subClassOf>
		<rdfs:label>dryland</rdfs:label>
		<skos:definition>land characterized by low rainfall, often used for agricultural purposes or recreation in deserts and other arid regions</skos:definition>
	</owl:Class>
	
	<owl:Class rdf:about="&oe-wtgw;Facility">
		<rdfs:label>facility</rdfs:label>
		<skos:definition>improvements and other material things provided for the use, accommodation, and convenience of park visitors</skos:definition>
	</owl:Class>
	
	<owl:Class rdf:about="&oe-wtgw;Fall">
		<rdfs:subClassOf rdf:resource="&oe-wtgw;Season"/>
		<rdfs:label>fall</rdfs:label>
		<skos:definition>temperatures drop, and many trees lose their leaves</skos:definition>
	</owl:Class>
	
	<owl:Class rdf:about="&oe-wtgw;GrayWolf">
		<rdfs:subClassOf rdf:resource="&oe-wtgw;Mammal"/>
		<rdfs:label>gray wolf</rdfs:label>
		<skos:definition>subclass of Mammal Class that describes a Gray Wolf</skos:definition>
	</owl:Class>
	
	<owl:Class rdf:about="&oe-wtgw;Habit">
		<rdfs:label>dietary habit</rdfs:label>
		<skos:definition>the natural environment in which a species or group of species lives and thrives, providing essential resources like food, shelter, and space</skos:definition>
	</owl:Class>
	
	<owl:Class rdf:about="&oe-wtgw;Herbivore">
		<rdfs:subClassOf rdf:resource="&oe-wtgw;DietaryPattern"/>
		<rdfs:label>herbivore</rdfs:label>
		<owl:disjointWith rdf:resource="&oe-wtgw;Omnivore"/>
		<skos:definition>an animal that only eats plant</skos:definition>
	</owl:Class>
	
	<owl:Class rdf:about="&oe-wtgw;Hike">
		<rdfs:subClassOf rdf:resource="&oe-wtgw;Activity"/>
		<rdfs:subClassOf>
			<owl:Restriction>
				<owl:onProperty rdf:resource="&oe-wtgw;hasDifficulty"/>
				<owl:someValuesFrom rdf:resource="&oe-wtgw;Difficulty"/>
			</owl:Restriction>
		</rdfs:subClassOf>
		<rdfs:subClassOf>
			<owl:Restriction>
				<owl:onProperty rdf:resource="&oe-wtgw;hasDistance"/>
				<owl:someValuesFrom rdf:resource="&xsd;float"/>
			</owl:Restriction>
		</rdfs:subClassOf>
		<rdfs:subClassOf>
			<owl:Restriction>
				<owl:onProperty rdf:resource="&oe-wtgw;isHikeOf"/>
				<owl:someValuesFrom rdf:resource="&oe-wtgw;NationalPark"/>
			</owl:Restriction>
		</rdfs:subClassOf>
		<rdfs:label>hike</rdfs:label>
		<skos:definition>a long walk, typically through countryside or wilderness areas, undertaken for leisure or exercise</skos:definition>
	</owl:Class>
	
	<owl:Class rdf:about="&oe-wtgw;Hotel">
		<rdfs:subClassOf rdf:resource="&oe-wtgw;Accomodation"/>
		<rdfs:label>hotel</rdfs:label>
		<skos:definition>buildings providing lodging, meals, and other services for travelers and tourists, often found near parks or recreational areas</skos:definition>
	</owl:Class>
	
	<owl:Class rdf:about="&oe-wtgw;IceLand">
		<rdfs:subClassOf rdf:resource="&oe-wtgw;Terrain"/>
		<rdfs:subClassOf>
			<owl:Restriction>
				<owl:onProperty rdf:resource="&oe-wtgw;hasClimate"/>
				<owl:someValuesFrom>
					<owl:Class>
						<owl:unionOf rdf:parseType="Collection">
							<rdf:Description rdf:about="&oe-wtgw;Cold">
							</rdf:Description>
							<rdf:Description rdf:about="&oe-wtgw;Rainy">
							</rdf:Description>
							<rdf:Description rdf:about="&oe-wtgw;Sunny">
							</rdf:Description>
							<rdf:Description rdf:about="&oe-wtgw;Windy">
							</rdf:Description>
						</owl:unionOf>
					</owl:Class>
				</owl:someValuesFrom>
			</owl:Restriction>
		</rdfs:subClassOf>
		<rdfs:label>ice land</rdfs:label>
		<skos:definition>a region characterized by permanent or seasonal ice and snow cover, such as glaciers or polar areas, offering unique ecosystems and recreational opportunities</skos:definition>
	</owl:Class>
	
	<owl:Class rdf:about="&oe-wtgw;InformationStation">
		<rdfs:subClassOf rdf:resource="&oe-wtgw;Facility"/>
		<rdfs:label>information station</rdfs:label>
		<skos:definition>a booth or building where visitors can receive assistance, guides, and information regarding their surroundings in parks, campsites, or other public areas</skos:definition>
	</owl:Class>
	
	<owl:Class rdf:about="&oe-wtgw;Insect">
		<rdfs:subClassOf rdf:resource="&oe-wtgw;Animal"/>
		<rdfs:label>insect</rdfs:label>
		<skos:definition>a small arthropod animal with a segmented body, six legs, and typically wings, such as flies, bees, and ants</skos:definition>
	</owl:Class>
	
	<owl:Class rdf:about="&oe-wtgw;License">
		<rdfs:subClassOf rdf:resource="&cmns-doc;LegalDocument"/>
		<rdfs:subClassOf>
			<owl:Restriction>
				<owl:onProperty rdf:resource="&cmns-pts;holdsDuring"/>
				<owl:onClass rdf:resource="&cmns-dt;DatePeriod"/>
				<owl:qualifiedCardinality rdf:datatype="&xsd;nonNegativeInteger">1</owl:qualifiedCardinality>
			</owl:Restriction>
		</rdfs:subClassOf>
		<rdfs:subClassOf>
			<owl:Restriction>
				<owl:onProperty rdf:resource="&oe-wtgw;isIssuedBy"/>
				<owl:someValuesFrom rdf:resource="&oe-wtgw;Licensor"/>
			</owl:Restriction>
		</rdfs:subClassOf>
		<rdfs:subClassOf>
			<owl:Restriction>
				<owl:onProperty rdf:resource="&cmns-pts;hasPartyRole"/>
				<owl:someValuesFrom rdf:resource="&oe-wtgw;Licensee"/>
			</owl:Restriction>
		</rdfs:subClassOf>
		<rdfs:label>license</rdfs:label>
		<skos:definition>grant of permission needed to do something</skos:definition>
		<cmns-av:adaptedFrom>Barron&apos;s Dictionary of Business and Economics Terms, Fifth Edition, 2012</cmns-av:adaptedFrom>
		<cmns-av:explanatoryNote>Note that in some cases, a license may also be considered an agreement or contract, depending on the specifics of the license and jurisdiction.</cmns-av:explanatoryNote>
	</owl:Class>
	
	<owl:Class rdf:about="&oe-wtgw;Licensee">
		<rdfs:subClassOf rdf:resource="&cmns-pts;PartyRole"/>
		<rdfs:subClassOf>
			<owl:Restriction>
				<owl:onProperty rdf:resource="&cmns-rlcmp;isPlayedBy"/>
				<owl:someValuesFrom>
					<owl:Restriction>
						<owl:onProperty rdf:resource="&cmns-pts;isAPartyTo"/>
						<owl:someValuesFrom rdf:resource="&oe-wtgw;License"/>
					</owl:Restriction>
				</owl:someValuesFrom>
			</owl:Restriction>
		</rdfs:subClassOf>
		<rdfs:label>licensee</rdfs:label>
		<skos:definition>a party to whom a license has been granted</skos:definition>
		<cmns-av:adaptedFrom>Barron&apos;s Dictionary of Business and Economics Terms, Fifth Edition, 2012</cmns-av:adaptedFrom>
	</owl:Class>
	
	<owl:Class rdf:about="&oe-wtgw;Licensor">
		<rdfs:subClassOf rdf:resource="&cmns-pts;PartyRole"/>
		<rdfs:subClassOf>
			<owl:Restriction>
				<owl:onProperty rdf:resource="&oe-wtgw;issues"/>
				<owl:someValuesFrom rdf:resource="&oe-wtgw;License"/>
			</owl:Restriction>
		</rdfs:subClassOf>
		<rdfs:subClassOf>
			<owl:Restriction>
				<owl:onProperty rdf:resource="&oe-wtgw;licenses"/>
				<owl:someValuesFrom rdf:resource="&owl;Thing"/>
			</owl:Restriction>
		</rdfs:subClassOf>
		<rdfs:subClassOf>
			<owl:Restriction>
				<owl:onProperty rdf:resource="&cmns-rlcmp;isPlayedBy"/>
				<owl:someValuesFrom>
					<owl:Restriction>
						<owl:onProperty rdf:resource="&cmns-pts;isAPartyTo"/>
						<owl:someValuesFrom rdf:resource="&oe-wtgw;License"/>
					</owl:Restriction>
				</owl:someValuesFrom>
			</owl:Restriction>
		</rdfs:subClassOf>
		<rdfs:label>licensor</rdfs:label>
		<skos:definition>a party who grants a license</skos:definition>
		<cmns-av:adaptedFrom>Barron&apos;s Dictionary of Business and Economics Terms, Fifth Edition, 2012</cmns-av:adaptedFrom>
	</owl:Class>
	
	<owl:Class rdf:about="&oe-wtgw;LoopTrail">
		<rdfs:subClassOf rdf:resource="&oe-wtgw;TrailType"/>
		<rdfs:label>loop trail</rdfs:label>
		<skos:definition>a trail that starts and ends at the same point forming a circular route</skos:definition>
	</owl:Class>
	
	<owl:Class rdf:about="&oe-wtgw;Mammal">
		<rdfs:subClassOf rdf:resource="&oe-wtgw;Animal"/>
		<rdfs:label>mammal</rdfs:label>
		<skos:definition>a warm-blooded vertebrate animal of a class that is distinguished by the presence of hair or fur, and females typically have mammary glands that produce milk for their young</skos:definition>
	</owl:Class>
	
	<owl:Class rdf:about="&oe-wtgw;Mountain">
		<rdfs:subClassOf rdf:resource="&oe-wtgw;Terrain"/>
		<rdfs:subClassOf>
			<owl:Restriction>
				<owl:onProperty rdf:resource="&oe-wtgw;hasClimate"/>
				<owl:someValuesFrom>
					<owl:Class>
						<owl:unionOf rdf:parseType="Collection">
							<rdf:Description rdf:about="&oe-wtgw;Cold">
							</rdf:Description>
							<rdf:Description rdf:about="&oe-wtgw;Rainy">
							</rdf:Description>
							<rdf:Description rdf:about="&oe-wtgw;Sunny">
							</rdf:Description>
							<rdf:Description rdf:about="&oe-wtgw;Windy">
							</rdf:Description>
						</owl:unionOf>
					</owl:Class>
				</owl:someValuesFrom>
			</owl:Restriction>
		</rdfs:subClassOf>
		<rdfs:label>mountain</rdfs:label>
		<skos:definition>a large natural elevation of the earth’s surface rising abruptly from the surrounding level, often forming prominent features in parks and wilderness areas</skos:definition>
	</owl:Class>
	
	<owl:Class rdf:about="&oe-wtgw;MountainGoat">
		<rdfs:subClassOf rdf:resource="&oe-wtgw;Mammal"/>
		<rdfs:label>mountain goat</rdfs:label>
		<skos:definition>subclass of Mammal Class that describes a Mountain Goat</skos:definition>
	</owl:Class>
	
	<owl:Class rdf:about="&oe-wtgw;MountainLion">
		<rdfs:subClassOf rdf:resource="&oe-wtgw;Mammal"/>
		<rdfs:label>mountain lion</rdfs:label>
		<skos:definition>subclass of Mammal Class that describes a Mountain Lion</skos:definition>
	</owl:Class>
	
	<owl:Class rdf:about="&oe-wtgw;MuleDeer">
		<rdfs:subClassOf rdf:resource="&oe-wtgw;Mammal"/>
		<rdfs:label>mule deer</rdfs:label>
		<skos:definition>subclass of Mammal Class that describes a Mule Deer</skos:definition>
	</owl:Class>
	
	<owl:Class rdf:about="&oe-wtgw;NationalPark">
		<rdfs:subClassOf>
			<owl:Restriction>
				<owl:onProperty rdf:resource="&oe-wtgw;hasClimate"/>
				<owl:allValuesFrom>
					<owl:Class>
						<owl:unionOf rdf:parseType="Collection">
							<rdf:Description rdf:about="&oe-wtgw;Cold">
							</rdf:Description>
							<rdf:Description rdf:about="&oe-wtgw;Rainy">
							</rdf:Description>
							<rdf:Description rdf:about="&oe-wtgw;Windy">
							</rdf:Description>
						</owl:unionOf>
					</owl:Class>
				</owl:allValuesFrom>
			</owl:Restriction>
		</rdfs:subClassOf>
		<rdfs:subClassOf>
			<owl:Restriction>
				<owl:onProperty rdf:resource="&oe-wtgw;hasTerrain"/>
				<owl:allValuesFrom>
					<owl:Class>
						<owl:unionOf rdf:parseType="Collection">
							<rdf:Description rdf:about="&oe-wtgw;Dryland">
							</rdf:Description>
							<rdf:Description rdf:about="&oe-wtgw;IceLand">
							</rdf:Description>
							<rdf:Description rdf:about="&oe-wtgw;Mountain">
							</rdf:Description>
							<rdf:Description rdf:about="&oe-wtgw;WetLand">
							</rdf:Description>
						</owl:unionOf>
					</owl:Class>
				</owl:allValuesFrom>
			</owl:Restriction>
		</rdfs:subClassOf>
		<rdfs:subClassOf>
			<owl:Restriction>
				<owl:onProperty rdf:resource="&oe-wtgw;hasAccomodation"/>
				<owl:onClass rdf:resource="&oe-wtgw;Accomodation"/>
				<owl:minQualifiedCardinality rdf:datatype="&xsd;nonNegativeInteger">0</owl:minQualifiedCardinality>
			</owl:Restriction>
		</rdfs:subClassOf>
		<rdfs:subClassOf>
			<owl:Restriction>
				<owl:onProperty rdf:resource="&oe-wtgw;hasActivity"/>
				<owl:someValuesFrom rdf:resource="&oe-wtgw;Activity"/>
			</owl:Restriction>
		</rdfs:subClassOf>
		<rdfs:subClassOf>
			<owl:Restriction>
				<owl:onProperty rdf:resource="&oe-wtgw;hasAnimal"/>
				<owl:someValuesFrom rdf:resource="&oe-wtgw;Animal"/>
			</owl:Restriction>
		</rdfs:subClassOf>
		<rdfs:subClassOf>
			<owl:Restriction>
				<owl:onProperty rdf:resource="&oe-wtgw;hasAvgSeasonalTemperature"/>
				<owl:someValuesFrom rdf:resource="&oe-wtgw;AvgSeasonalTemperature"/>
			</owl:Restriction>
		</rdfs:subClassOf>
		<rdfs:subClassOf>
			<owl:Restriction>
				<owl:onProperty rdf:resource="&oe-wtgw;hasFacility"/>
				<owl:someValuesFrom rdf:resource="&oe-wtgw;Facility"/>
			</owl:Restriction>
		</rdfs:subClassOf>
		<rdfs:subClassOf>
			<owl:Restriction>
				<owl:onProperty rdf:resource="&oe-wtgw;hasParkStatistic"/>
				<owl:someValuesFrom rdf:resource="&oe-wtgw;ParkStatistic"/>
			</owl:Restriction>
		</rdfs:subClassOf>
		<rdfs:subClassOf>
			<owl:Restriction>
				<owl:onProperty rdf:resource="https://www.omg.org/spec/Commons/Locations/hasLocation"/>
				<owl:someValuesFrom rdf:resource="https://www.omg.org/spec/Commons/Locations/Location"/>
			</owl:Restriction>
		</rdfs:subClassOf>
		<rdfs:label>national park</rdfs:label>
		<skos:definition>a large area of land or water that is protected by a government for the preservation of its natural environment, history, or culture</skos:definition>
	</owl:Class>
	
	<owl:Class rdf:about="&oe-wtgw;NatureWalk">
		<rdfs:subClassOf rdf:resource="&oe-wtgw;Activity"/>
		<rdfs:label>nature walk</rdfs:label>
		<skos:definition>a walk on a nature trail, especially with an experienced guide</skos:definition>
	</owl:Class>
	
	<owl:Class rdf:about="&oe-wtgw;Omnivore">
		<rdfs:subClassOf rdf:resource="&oe-wtgw;DietaryPattern"/>
		<rdfs:label>omnivore</rdfs:label>
		<skos:definition>an animal that eats both plants and other animals</skos:definition>
	</owl:Class>
	
	<owl:Class rdf:about="&oe-wtgw;OutandBackTrail">
		<rdfs:subClassOf rdf:resource="&oe-wtgw;TrailType"/>
		<rdfs:label>outand back trail</rdfs:label>
		<skos:definition>a trail that starts in one spot and ends in another, hikers will have to retrace their footsteps or find another trail back to where they started</skos:definition>
	</owl:Class>
	
	<owl:Class rdf:about="&oe-wtgw;ParkStatistic">
		<rdfs:label>park statistic</rdfs:label>
		<skos:definition>statistics about a park, including visitation numbers, trail usage, wildlife sightings, and other relevant data to monitor park activity and health</skos:definition>
	</owl:Class>
	
	<owl:Class rdf:about="&oe-wtgw;Parking">
		<rdfs:subClassOf rdf:resource="&oe-wtgw;Facility"/>
		<rdfs:label>parking</rdfs:label>
		<skos:definition>a space or lot where vehicles can be parked, typically found at entrances to parks, trails, or campsites</skos:definition>
	</owl:Class>
	
	<owl:Class rdf:about="&oe-wtgw;Rainy">
		<rdfs:subClassOf rdf:resource="&oe-wtgw;Climate"/>
		<rdfs:label>rainy</rdfs:label>
		<owl:disjointWith rdf:resource="&oe-wtgw;Sunny"/>
		<skos:definition>marked by more rain than usual</skos:definition>
	</owl:Class>
	
	<owl:Class rdf:about="&oe-wtgw;Reptile">
		<rdfs:subClassOf rdf:resource="&oe-wtgw;Animal"/>
		<rdfs:label>reptile</rdfs:label>
		<skos:definition>a cold-blooded vertebrate animal that has dry, scaly skin and typically lays soft-shelled eggs on land, such as snakes, lizards, and turtles</skos:definition>
	</owl:Class>
	
	<owl:Class rdf:about="&oe-wtgw;Season">
		<rdfs:label>season</rdfs:label>
		<skos:definition>each of the four divisions of the year (spring, summer, fall, and winter) marked by particular weather patterns and daylight hours, resulting from the earth&apos;s changing position with regard to the sun</skos:definition>
	</owl:Class>
	
	<owl:Class rdf:about="&oe-wtgw;Spring">
		<rdfs:subClassOf rdf:resource="&oe-wtgw;Season"/>
		<rdfs:label>spring</rdfs:label>
		<skos:definition>is when plants sprout, tree leaves unfurl, and flowers blossom</skos:definition>
	</owl:Class>
	
	<owl:Class rdf:about="&oe-wtgw;State">
		<rdfs:subClassOf rdf:resource="https://www.omg.org/spec/Commons/Locations/Location"/>
		<rdfs:label>state</rdfs:label>
		<skos:definition>the 50 territories that make up the United States of America</skos:definition>
	</owl:Class>
	
	<owl:Class rdf:about="&oe-wtgw;Summer">
		<rdfs:subClassOf rdf:resource="&oe-wtgw;Season"/>
		<rdfs:label>summer</rdfs:label>
		<skos:definition>is the warmest time of the year and has the most daylight, so plants grow quickly</skos:definition>
	</owl:Class>
	
	<owl:Class rdf:about="&oe-wtgw;Sunny">
		<rdfs:subClassOf rdf:resource="&oe-wtgw;Climate"/>
		<rdfs:label>sunny</rdfs:label>
		<skos:definition>exposed to, brightened by, or warmed by the sun</skos:definition>
	</owl:Class>
	
	<owl:Class rdf:about="&oe-wtgw;Terrain">
		<rdfs:label>terrain</rdfs:label>
		<skos:definition>the physical features of a piece of land, including its elevation, slope, and orientation, often used to describe hiking or camping environments</skos:definition>
	</owl:Class>
	
	<owl:Class rdf:about="&oe-wtgw;TrailType">
		<rdfs:label>trail type</rdfs:label>
		<skos:definition>a category of trail based on observable patterns in the trail</skos:definition>
	</owl:Class>
	
	<owl:Class rdf:about="&oe-wtgw;WesternRattlesnake">
		<rdfs:subClassOf rdf:resource="&oe-wtgw;Reptile"/>
		<rdfs:label>western rattlesnake</rdfs:label>
		<skos:definition>subclass of Reptile Class that describes a Western Rattlesnake</skos:definition>
	</owl:Class>
	
	<owl:Class rdf:about="&oe-wtgw;WetLand">
		<rdfs:subClassOf rdf:resource="&oe-wtgw;Terrain"/>
		<rdfs:subClassOf>
			<owl:Restriction>
				<owl:onProperty rdf:resource="&oe-wtgw;hasClimate"/>
				<owl:someValuesFrom>
					<owl:Class>
						<owl:unionOf rdf:parseType="Collection">
							<rdf:Description rdf:about="&oe-wtgw;Rainy">
							</rdf:Description>
							<rdf:Description rdf:about="&oe-wtgw;Sunny">
							</rdf:Description>
							<rdf:Description rdf:about="&oe-wtgw;Windy">
							</rdf:Description>
						</owl:unionOf>
					</owl:Class>
				</owl:someValuesFrom>
			</owl:Restriction>
		</rdfs:subClassOf>
		<rdfs:label>wet land</rdfs:label>
		<skos:definition>an area of land that is saturated with water either permanently or seasonally, such as marshes, swamps, and bogs, providing unique ecosystems</skos:definition>
	</owl:Class>
	
	<owl:Class rdf:about="&oe-wtgw;Windy">
		<rdfs:subClassOf rdf:resource="&oe-wtgw;Climate"/>
		<rdfs:label>windy</rdfs:label>
		<skos:definition>marked by strong wind or by more wind than usual</skos:definition>
	</owl:Class>
	
	<owl:Class rdf:about="&oe-wtgw;Winter">
		<rdfs:subClassOf rdf:resource="&oe-wtgw;Season"/>
		<rdfs:label>winter</rdfs:label>
		<skos:definition>typically has cold weather, little daylight, and limited plant growth</skos:definition>
	</owl:Class>
	
	<owl:ObjectProperty rdf:about="&oe-wtgw;hasAccessibility">
		<rdfs:label>has accessibility</rdfs:label>
		<rdfs:domain rdf:resource="&oe-wtgw;Facility"/>
		<rdfs:domain rdf:resource="&oe-wtgw;NationalPark"/>
		<skos:definition>the degree to which a park, trail, or facility is accessible to individuals with disabilities, including features like ramps, designated parking, and trail modifications</skos:definition>
	</owl:ObjectProperty>
	
	<owl:ObjectProperty rdf:about="&oe-wtgw;hasAccomodation">
		<rdfs:label>has accomodation</rdfs:label>
		<rdfs:domain rdf:resource="&oe-wtgw;NationalPark"/>
		<skos:definition>temporary lodgings, sometimes also including board</skos:definition>
	</owl:ObjectProperty>
	
	<owl:ObjectProperty rdf:about="&oe-wtgw;hasActivity">
		<rdfs:label>has activity</rdfs:label>
		<rdfs:domain rdf:resource="&oe-wtgw;NationalPark"/>
		<rdfs:range rdf:resource="&oe-wtgw;Activity"/>
		<skos:definition>a use of the park by visitors</skos:definition>
	</owl:ObjectProperty>
	
	<owl:ObjectProperty rdf:about="&oe-wtgw;hasAnimal">
		<rdfs:label>has animal</rdfs:label>
		<rdfs:domain rdf:resource="&oe-wtgw;NationalPark"/>
		<rdfs:range rdf:resource="&oe-wtgw;Animal"/>
		<skos:definition>a living organism that feeds on organic matter, typically having specialized sense organs and nervous systems and able to move voluntarily</skos:definition>
	</owl:ObjectProperty>
	
	<owl:ObjectProperty rdf:about="&oe-wtgw;hasAvgSeasonalTemperature">
		<rdfs:label>has average seasonal temperature</rdfs:label>
		<rdfs:domain rdf:resource="&oe-wtgw;NationalPark"/>
		<rdfs:range rdf:resource="&oe-wtgw;Season"/>
		<skos:definition>the mean thermal reading of a specific place over a part of the year</skos:definition>
	</owl:ObjectProperty>
	
	<owl:ObjectProperty rdf:about="&oe-wtgw;hasCapacity">
		<rdfs:label>hasCapacity</rdfs:label>
		<rdfs:domain rdf:resource="&oe-wtgw;Facility"/>
		<skos:definition>The maximum number of people, vehicles, or visitors that a park, campground, or facility can accommodate at one time.</skos:definition>
	</owl:ObjectProperty>
	
	<owl:ObjectProperty rdf:about="&oe-wtgw;hasClimate">
		<rdfs:label>has climate</rdfs:label>
		<rdfs:label>has temperature</rdfs:label>
		<rdfs:domain rdf:resource="&oe-wtgw;NationalPark"/>
		<rdfs:range rdf:resource="&oe-wtgw;Climate"/>
		<skos:definition>a measure of the warmth or coldness of an environment or substance, typically expressed in degrees Celsius or Fahrenheit</skos:definition>
		<skos:definition>the average weather conditions in a particular region over a long period, including temperature, humidity, wind patterns, and precipitation</skos:definition>
	</owl:ObjectProperty>
	
	<owl:ObjectProperty rdf:about="&oe-wtgw;hasDietaryPattern">
		<rdfs:label>has dietary pattern</rdfs:label>
		<rdfs:domain rdf:resource="&oe-wtgw;Animal"/>
		<rdfs:range rdf:resource="&oe-wtgw;DietaryPattern"/>
		<skos:definition>the habitual eating behaviors and food choices of an individual or group, often categorized by food type, frequency, and portion size</skos:definition>
	</owl:ObjectProperty>
	
	<owl:ObjectProperty rdf:about="&oe-wtgw;hasDifficulty">
		<rdfs:label>has difficulty</rdfs:label>
		<rdfs:domain rdf:resource="&oe-wtgw;Hike"/>
		<rdfs:range rdf:resource="&oe-wtgw;Difficulty"/>
		<skos:definition>Property describing if a trail has a difficulty rating</skos:definition>
	</owl:ObjectProperty>
	
	<owl:DatatypeProperty rdf:about="&oe-wtgw;hasDistance">
		<rdfs:subPropertyOf rdf:resource="https://www.omg.org/spec/Commons/QuantitiesAndUnits/hasNumericValue"/>
		<rdfs:comment>has distance</rdfs:comment>
		<rdfs:range>
			<rdfs:Datatype>
				<owl:onDatatype rdf:resource="&xsd;decimal"/>
				<owl:withRestrictions rdf:parseType="Collection">
					<rdf:Description>
						<xsd:minInclusive rdf:datatype="&xsd;decimal">0</xsd:minInclusive>
					</rdf:Description>
				</owl:withRestrictions>
			</rdfs:Datatype>
		</rdfs:range>
		<skos:definition>the amount of space between two points</skos:definition>
	</owl:DatatypeProperty>
	
	<owl:ObjectProperty rdf:about="&oe-wtgw;hasFacility">
		<rdfs:label>has facility</rdfs:label>
		<rdfs:domain rdf:resource="&oe-wtgw;NationalPark"/>
		<rdfs:range rdf:resource="&oe-wtgw;Facility"/>
		<skos:definition>improvements and other material things provided for the use, accommodation, and convenience of park visitors</skos:definition>
	</owl:ObjectProperty>
	
	<owl:ObjectProperty rdf:about="&oe-wtgw;hasHabit">
		<rdfs:label>has habit</rdfs:label>
		<skos:definition>the natural environment in which a species or group of species lives and thrives, providing essential resources like food, shelter, and space</skos:definition>
	</owl:ObjectProperty>
	
	<owl:ObjectProperty rdf:about="&oe-wtgw;hasHike">
		<rdfs:subPropertyOf rdf:resource="&oe-wtgw;hasActivity"/>
		<rdfs:label>has hike</rdfs:label>
		<rdfs:domain rdf:resource="&oe-wtgw;NationalPark"/>
		<rdfs:range rdf:resource="&oe-wtgw;Hike"/>
		<skos:definition>a long walk, typically through countryside or wilderness areas, undertaken for leisure or exercise</skos:definition>
	</owl:ObjectProperty>
	
	<owl:ObjectProperty rdf:about="&oe-wtgw;hasHumidity">
		<rdfs:label>has humidity</rdfs:label>
		<rdfs:domain rdf:resource="&oe-wtgw;NationalPark"/>
		<rdfs:range>
			<owl:Restriction>
				<owl:onProperty rdf:resource="https://www.omg.org/spec/Commons/QuantitiesAndUnits/hasNumericValue"/>
				<owl:someValuesFrom rdf:resource="&xsd;float"/>
			</owl:Restriction>
		</rdfs:range>
		<skos:definition>the amount of water vapor present in the air, expressed as a percentage, influencing comfort levels and weather patterns</skos:definition>
	</owl:ObjectProperty>
	
	<owl:ObjectProperty rdf:about="&oe-wtgw;hasParkStatistic">
		<rdfs:label>has park statistic</rdfs:label>
		<rdfs:domain rdf:resource="&oe-wtgw;NationalPark"/>
		<rdfs:range rdf:resource="&oe-wtgw;ParkStatistic"/>
		<skos:definition>statistics about a park, including visitation numbers, trail usage, wildlife sightings, and other relevant data to monitor park activity and health</skos:definition>
	</owl:ObjectProperty>
	
	<owl:ObjectProperty rdf:about="&oe-wtgw;hasSeason">
		<rdfs:label>has season</rdfs:label>
		<rdfs:range rdf:resource="&oe-wtgw;Season"/>
		<skos:definition>each of the four divisions of the year (spring, summer, fall, and winter) marked by particular weather patterns and daylight hours, resulting from the earth&apos;s changing position with regard to the sun</skos:definition>
	</owl:ObjectProperty>
	
	<owl:DatatypeProperty rdf:about="&oe-wtgw;hasTemperature">
		<rdfs:subPropertyOf rdf:resource="https://www.omg.org/spec/Commons/QuantitiesAndUnits/hasNumericValue"/>
		<rdfs:label>has temperature</rdfs:label>
		<skos:definition>the thermal reading of a specific place</skos:definition>
	</owl:DatatypeProperty>
	
	<owl:ObjectProperty rdf:about="&oe-wtgw;hasTerrain">
		<rdfs:subPropertyOf rdf:resource="&oe-wtgw;temperatureHasSeason"/>
		<rdfs:label>terrain</rdfs:label>
		<rdfs:domain rdf:resource="&oe-wtgw;NationalPark"/>
		<rdfs:range rdf:resource="&oe-wtgw;Terrain"/>
		<skos:definition>the physical features of a piece of land, including its elevation, slope, and orientation, often used to describe hiking or camping environments</skos:definition>
	</owl:ObjectProperty>
	
	<owl:ObjectProperty rdf:about="&oe-wtgw;hasTrailHead">
		<rdfs:label>has trail head</rdfs:label>
		<rdfs:domain rdf:resource="&oe-wtgw;Hike"/>
		<skos:definition>the start of a trail</skos:definition>
	</owl:ObjectProperty>
	
	<owl:ObjectProperty rdf:about="&oe-wtgw;hasTrailType">
		<rdfs:label>has trail type</rdfs:label>
		<rdfs:domain rdf:resource="&oe-wtgw;Hike"/>
		<rdfs:range rdf:resource="&oe-wtgw;TrailType"/>
		<skos:definition>the kind of trail it is, can either be out and back or a loop</skos:definition>
	</owl:ObjectProperty>
	
	<owl:ObjectProperty rdf:about="&oe-wtgw;isHikeOf">
		<rdfs:domain rdf:resource="&oe-wtgw;Hike"/>
		<rdfs:range rdf:resource="&oe-wtgw;NationalPark"/>
	</owl:ObjectProperty>
	
	<owl:ObjectProperty rdf:about="&oe-wtgw;isIssuedBy">
		<rdfs:subPropertyOf rdf:resource="&cmns-org;isProvidedBy"/>
		<rdfs:label>is issued by</rdfs:label>
		<rdfs:range rdf:resource="&cmns-pts;AgentRole"/>
		<owl:inverseOf rdf:resource="&oe-wtgw;issues"/>
		<skos:definition>indicates a role played by a functional entity or party responsible for circulating, distributing, or publishing something</skos:definition>
	</owl:ObjectProperty>
	
	<owl:ObjectProperty rdf:about="&oe-wtgw;issues">
		<rdfs:subPropertyOf rdf:resource="&cmns-org;provides"/>
		<rdfs:label>issues</rdfs:label>
		<rdfs:domain rdf:resource="&cmns-pts;AgentRole"/>
		<skos:definition>officially makes something available</skos:definition>
	</owl:ObjectProperty>
	
	<owl:ObjectProperty rdf:about="&oe-wtgw;licenses">
		<rdfs:label>licenses</rdfs:label>
		<skos:definition>grant of permission needed to do something</skos:definition>
	</owl:ObjectProperty>
	
	<owl:ObjectProperty rdf:about="&oe-wtgw;temperatureHasSeason">
		<rdfs:subPropertyOf rdf:resource="&oe-wtgw;hasSeason"/>
		<rdfs:label>temperature has season</rdfs:label>
		<rdfs:domain rdf:resource="&oe-wtgw;AvgSeasonalTemperature"/>
		<rdfs:range rdf:resource="&oe-wtgw;Season"/>
		<skos:definition>the thermal reading of each of the four divisions of the year (spring, summer, fall, and winter) marked by particular weather patterns and daylight hours, resulting from the earth&apos;s changing position with regard to the sun</skos:definition>
	</owl:ObjectProperty>
	
	<rdf:Description rdf:about="https://www.omg.org/spec/Commons/Locations/PhysicalLocation">
		<rdfs:subClassOf>
			<owl:Restriction>
				<owl:onProperty rdf:resource="https://www.omg.org/spec/Commons/Locations/hasLatitude"/>
				<owl:someValuesFrom rdf:resource="&xsd;long"/>
			</owl:Restriction>
		</rdfs:subClassOf>
		<rdfs:subClassOf>
			<owl:Restriction>
				<owl:onProperty rdf:resource="https://www.omg.org/spec/Commons/Locations/hasLongitude"/>
				<owl:someValuesFrom rdf:resource="&xsd;long"/>
			</owl:Restriction>
		</rdfs:subClassOf>
	</rdf:Description>
	
	<owl:ObjectProperty rdf:about="&cmns-org;isProvidedBy">
	</owl:ObjectProperty>
	
	<owl:ObjectProperty rdf:about="&cmns-org;provides">
	</owl:ObjectProperty>
	
	<rdf:Description rdf:about="&cmns-pts;Situation">
		<rdfs:subClassOf rdf:resource="https://www.omg.org/spec/Commons/QuantitiesAndUnits/ScalarQuantity"/>
	</rdf:Description>

</rdf:RDF>