<?xml version="1.0" encoding="UTF-8"?>
<!DOCTYPE rdf:RDF [
	<!ENTITY dct "http://purl.org/dc/terms/">
	<!ENTITY fibo-fnd-aap-ppl "https://spec.edmcouncil.org/fibo/ontology/FND/AgentsAndPeople/People/">
	<!ENTITY fibo-fnd-arr-arr "https://spec.edmcouncil.org/fibo/ontology/FND/Arrangements/Arrangements/">
	<!ENTITY fibo-fnd-arr-cls "https://spec.edmcouncil.org/fibo/ontology/FND/Arrangements/ClassificationSchemes/">
	<!ENTITY fibo-fnd-dt-fd "https://spec.edmcouncil.org/fibo/ontology/FND/DatesAndTimes/FinancialDates/">
	<!ENTITY fibo-fnd-org-fm "https://spec.edmcouncil.org/fibo/ontology/FND/Organizations/FormalOrganizations/">
	<!ENTITY fibo-fnd-pas-pas "https://spec.edmcouncil.org/fibo/ontology/FND/ProductsAndServices/ProductsAndServices/">
	<!ENTITY fibo-fnd-pty-pty "https://spec.edmcouncil.org/fibo/ontology/FND/Parties/Parties/">
	<!ENTITY fibo-fnd-pty-rl "https://spec.edmcouncil.org/fibo/ontology/FND/Parties/Roles/">
	<!ENTITY fibo-fnd-qt-qtu "https://spec.edmcouncil.org/fibo/ontology/FND/Quantities/QuantitiesAndUnits/">
	<!ENTITY fibo-fnd-rel-rel "https://spec.edmcouncil.org/fibo/ontology/FND/Relations/Relations/">
	<!ENTITY fibo-fnd-utl-alx "https://spec.edmcouncil.org/fibo/ontology/FND/Utilities/Analytics/">
	<!ENTITY fibo-fnd-utl-av "https://spec.edmcouncil.org/fibo/ontology/FND/Utilities/AnnotationVocabulary/">
	<!ENTITY lcc-cr "https://www.omg.org/spec/LCC/Countries/CountryRepresentation/">
	<!ENTITY lcc-lr "https://www.omg.org/spec/LCC/Languages/LanguageRepresentation/">
	<!ENTITY oe2020-pat-rec "https://tw.rpi.edu/ontology-engineering/oe2020/patient-guideline-recommender/">
	<!ENTITY owl "http://www.w3.org/2002/07/owl#">
	<!ENTITY rdf "http://www.w3.org/1999/02/22-rdf-syntax-ns#">
	<!ENTITY rdfs "http://www.w3.org/2000/01/rdf-schema#">
	<!ENTITY skos "http://www.w3.org/2004/02/skos/core#">
	<!ENTITY sm "http://www.omg.org/techprocess/ab/SpecificationMetadata/">
	<!ENTITY xsd "http://www.w3.org/2001/XMLSchema#">
]>
<rdf:RDF xml:base="https://tw.rpi.edu/ontology-engineering/oe2020/patient-guideline-recommender/"
	xmlns:dct="http://purl.org/dc/terms/"
	xmlns:fibo-fnd-aap-ppl="https://spec.edmcouncil.org/fibo/ontology/FND/AgentsAndPeople/People/"
	xmlns:fibo-fnd-arr-arr="https://spec.edmcouncil.org/fibo/ontology/FND/Arrangements/Arrangements/"
	xmlns:fibo-fnd-arr-cls="https://spec.edmcouncil.org/fibo/ontology/FND/Arrangements/ClassificationSchemes/"
	xmlns:fibo-fnd-dt-fd="https://spec.edmcouncil.org/fibo/ontology/FND/DatesAndTimes/FinancialDates/"
	xmlns:fibo-fnd-org-fm="https://spec.edmcouncil.org/fibo/ontology/FND/Organizations/FormalOrganizations/"
	xmlns:fibo-fnd-pas-pas="https://spec.edmcouncil.org/fibo/ontology/FND/ProductsAndServices/ProductsAndServices/"
	xmlns:fibo-fnd-pty-pty="https://spec.edmcouncil.org/fibo/ontology/FND/Parties/Parties/"
	xmlns:fibo-fnd-pty-rl="https://spec.edmcouncil.org/fibo/ontology/FND/Parties/Roles/"
	xmlns:fibo-fnd-qt-qtu="https://spec.edmcouncil.org/fibo/ontology/FND/Quantities/QuantitiesAndUnits/"
	xmlns:fibo-fnd-rel-rel="https://spec.edmcouncil.org/fibo/ontology/FND/Relations/Relations/"
	xmlns:fibo-fnd-utl-alx="https://spec.edmcouncil.org/fibo/ontology/FND/Utilities/Analytics/"
	xmlns:fibo-fnd-utl-av="https://spec.edmcouncil.org/fibo/ontology/FND/Utilities/AnnotationVocabulary/"
	xmlns:lcc-cr="https://www.omg.org/spec/LCC/Countries/CountryRepresentation/"
	xmlns:lcc-lr="https://www.omg.org/spec/LCC/Languages/LanguageRepresentation/"
	xmlns:oe2020-pat-rec="https://tw.rpi.edu/ontology-engineering/oe2020/patient-guideline-recommender/"
	xmlns:owl="http://www.w3.org/2002/07/owl#"
	xmlns:rdf="http://www.w3.org/1999/02/22-rdf-syntax-ns#"
	xmlns:rdfs="http://www.w3.org/2000/01/rdf-schema#"
	xmlns:skos="http://www.w3.org/2004/02/skos/core#"
	xmlns:sm="http://www.omg.org/techprocess/ab/SpecificationMetadata/"
	xmlns:xsd="http://www.w3.org/2001/XMLSchema#">
	
	<owl:Ontology rdf:about="https://tw.rpi.edu/ontology-engineering/oe2020/patient-guideline-recommender/">
		<rdfs:label>Patient Guideline Recommender Ontology</rdfs:label>
		<dct:abstract>The goal of this project is to provide the tools to assess the nutritional/lifestyle needs of a diabetic patient. We would do this by developing an ontology-enabled application that would use the ontology tocould answer patient questions based on the recommendations detailed in the authoritative literature in the diabetes domain, the Standards of Medical Care, Clinical Practice Guidelines (CPG) released by the American Diabetes Association (ADA). The ontology should also match them to the guidelines that are relevant to them.</dct:abstract>
		<dct:creator>Ishita Padhiar</dct:creator>
		<dct:creator>Liam Feehery</dct:creator>
		<dct:creator>Namir Xia</dct:creator>
		<dct:creator>Travis Peterson</dct:creator>
		<sm:dependsOn rdf:datatype="&xsd;anyURI">https://spec.edmcouncil.org/fibo/ontology/FND/</sm:dependsOn>
		<sm:dependsOn rdf:datatype="&xsd;anyURI">https://www.omg.org/spec/LCC/</sm:dependsOn>
		<owl:imports rdf:resource="https://spec.edmcouncil.org/fibo/ontology/FND/AgentsAndPeople/People/"/>
		<owl:imports rdf:resource="https://spec.edmcouncil.org/fibo/ontology/FND/Arrangements/Arrangements/"/>
		<owl:imports rdf:resource="https://spec.edmcouncil.org/fibo/ontology/FND/Arrangements/ClassificationSchemes/"/>
		<owl:imports rdf:resource="https://spec.edmcouncil.org/fibo/ontology/FND/DatesAndTimes/FinancialDates/"/>
		<owl:imports rdf:resource="https://spec.edmcouncil.org/fibo/ontology/FND/GoalsAndObjectives/Objectives/"/>
		<owl:imports rdf:resource="https://spec.edmcouncil.org/fibo/ontology/FND/Organizations/FormalOrganizations/"/>
		<owl:imports rdf:resource="https://spec.edmcouncil.org/fibo/ontology/FND/Parties/Parties/"/>
		<owl:imports rdf:resource="https://spec.edmcouncil.org/fibo/ontology/FND/Parties/Roles/"/>
		<owl:imports rdf:resource="https://spec.edmcouncil.org/fibo/ontology/FND/ProductsAndServices/ProductsAndServices/"/>
		<owl:imports rdf:resource="https://spec.edmcouncil.org/fibo/ontology/FND/Quantities/QuantitiesAndUnits/"/>
		<owl:imports rdf:resource="https://spec.edmcouncil.org/fibo/ontology/FND/Relations/Relations/"/>
		<owl:imports rdf:resource="https://spec.edmcouncil.org/fibo/ontology/FND/Utilities/Analytics/"/>
		<owl:imports rdf:resource="https://spec.edmcouncil.org/fibo/ontology/FND/Utilities/AnnotationVocabulary/"/>
		<owl:imports rdf:resource="https://www.omg.org/spec/LCC/Countries/CountryRepresentation/"/>
		<owl:imports rdf:resource="https://www.omg.org/spec/LCC/Languages/LanguageRepresentation/"/>
		<owl:versionIRI rdf:resource="https://tw.rpi.edu/ontology-engineering/oe2020/20201025/patient-guideline-recommender/"/>
	</owl:Ontology>
	
	<owl:Class rdf:about="&fibo-fnd-aap-ppl;DateOfBirth">
	</owl:Class>
	
	<owl:Class rdf:about="&fibo-fnd-aap-ppl;Person">
		<rdfs:subClassOf>
			<owl:Restriction>
				<owl:onProperty rdf:resource="&oe2020-pat-rec;eats"/>
				<owl:someValuesFrom rdf:resource="&oe2020-pat-rec;Food"/>
			</owl:Restriction>
		</rdfs:subClassOf>
		<rdfs:subClassOf>
			<owl:Restriction>
				<owl:onProperty rdf:resource="&oe2020-pat-rec;hasAge"/>
				<owl:someValuesFrom rdf:resource="&oe2020-pat-rec;PersonAge"/>
			</owl:Restriction>
		</rdfs:subClassOf>
		<rdfs:subClassOf>
			<owl:Restriction>
				<owl:onProperty rdf:resource="&oe2020-pat-rec;hasGenderIdentity"/>
				<owl:someValuesFrom rdf:resource="&oe2020-pat-rec;GenderIdentity"/>
			</owl:Restriction>
		</rdfs:subClassOf>
	</owl:Class>
	
	<owl:Class rdf:about="https://spec.edmcouncil.org/fibo/ontology/FND/GoalsAndObjectives/Objectives/Objective">
	</owl:Class>
	
	<owl:Class rdf:about="&oe2020-pat-rec;A1c">
		<rdfs:subClassOf rdf:resource="&fibo-fnd-qt-qtu;QuantityValue"/>
		<rdfs:subClassOf>
			<owl:Restriction>
				<owl:onProperty rdf:resource="&oe2020-pat-rec;isRiskFactorFor"/>
				<owl:someValuesFrom rdf:resource="&oe2020-pat-rec;Type2Diabetes"/>
			</owl:Restriction>
		</rdfs:subClassOf>
		<rdfs:label>a1c</rdfs:label>
		<skos:definition>a test that measures the level of hemoglobin A1c in the blood as a means of determining the average blood sugar concentrations for the preceding two to three months</skos:definition>
	</owl:Class>
	
	<owl:Class rdf:about="&oe2020-pat-rec;Active">
		<rdfs:subClassOf rdf:resource="&oe2020-pat-rec;ActivityLevel"/>
		<rdfs:label>active</rdfs:label>
		<skos:definition>requiring vigorous action or exertion</skos:definition>
	</owl:Class>
	
	<owl:Class rdf:about="&oe2020-pat-rec;ActivityLevel">
		<rdfs:subClassOf>
			<owl:Restriction>
				<owl:onProperty rdf:resource="&fibo-fnd-arr-arr;isConstituentOf"/>
				<owl:someValuesFrom rdf:resource="&oe2020-pat-rec;Lifestyle"/>
			</owl:Restriction>
		</rdfs:subClassOf>
		<rdfs:label>activity level</rdfs:label>
		<skos:definition>a way to express a person&apos;s daily physical activity as a number, and is used to estimate a person&apos;s total energy expenditure</skos:definition>
	</owl:Class>
	
	<owl:Class rdf:about="&oe2020-pat-rec;AerobicExercise">
		<rdfs:subClassOf rdf:resource="&oe2020-pat-rec;Exercise"/>
		<rdfs:label>aerobic exercise</rdfs:label>
		<skos:definition>physical exercise that depends primarily on the aerobic energy-generating process</skos:definition>
	</owl:Class>
	
	<owl:Class rdf:about="&oe2020-pat-rec;Age">
		<rdfs:subClassOf rdf:resource="&fibo-fnd-qt-qtu;QuantityValue"/>
		<rdfs:subClassOf rdf:resource="&fibo-fnd-utl-alx;Aspect"/>
		<rdfs:label>age</rdfs:label>
		<skos:definition>the number of full years, months, days, hours, etc., that someone, or something, has been alive</skos:definition>
	</owl:Class>
	
	<owl:Class rdf:about="&oe2020-pat-rec;AgeGroup">
		<rdfs:subClassOf rdf:resource="&oe2020-pat-rec;Demographic"/>
		<rdfs:label>age group</rdfs:label>
		<skos:definition>demographic indicating a range of ages that a member of a population falls in at some point in time</skos:definition>
	</owl:Class>
	
	<owl:Class rdf:about="&oe2020-pat-rec;BloodPressure">
		<rdfs:subClassOf rdf:resource="&fibo-fnd-qt-qtu;QuantityValue"/>
		<rdfs:label>blood pressure</rdfs:label>
		<skos:definition>the pressure of the circulating blood against the walls of the blood vessels</skos:definition>
	</owl:Class>
	
	<owl:Class rdf:about="&oe2020-pat-rec;BloodSugar">
		<rdfs:subClassOf rdf:resource="&fibo-fnd-qt-qtu;QuantityValue"/>
		<rdfs:subClassOf>
			<owl:Restriction>
				<owl:onProperty rdf:resource="&oe2020-pat-rec;isRiskFactorFor"/>
				<owl:someValuesFrom rdf:resource="&oe2020-pat-rec;Diabetes"/>
			</owl:Restriction>
		</rdfs:subClassOf>
		<rdfs:label>blood sugar</rdfs:label>
		<skos:definition>the glucose in the blood; also, its concentration</skos:definition>
	</owl:Class>
	
	<owl:Class rdf:about="&oe2020-pat-rec;BodyMass">
		<rdfs:subClassOf rdf:resource="&fibo-fnd-qt-qtu;QuantityValue"/>
		<rdfs:subClassOf>
			<owl:Restriction>
				<owl:onProperty rdf:resource="&oe2020-pat-rec;isRiskFactorFor"/>
				<owl:someValuesFrom rdf:resource="&oe2020-pat-rec;Obesity"/>
			</owl:Restriction>
		</rdfs:subClassOf>
		<rdfs:label>body mass</rdfs:label>
		<skos:definition>a measure of body fat that is the ratio of the weight of the body in kilograms to the square of its height in meters</skos:definition>
	</owl:Class>
	
	<owl:Class rdf:about="&oe2020-pat-rec;BodyWeightExercise">
		<rdfs:subClassOf rdf:resource="&oe2020-pat-rec;Exercise"/>
		<rdfs:label>body weight exercise</rdfs:label>
		<skos:definition>strength-training exercises that use the individual&apos;s own weight to provide resistance against gravity</skos:definition>
	</owl:Class>
	
	<owl:NamedIndividual rdf:about="&oe2020-pat-rec;Calorie">
		<rdf:type rdf:resource="&fibo-fnd-qt-qtu;DerivedUnit"/>
		<rdfs:label>Calorie</rdfs:label>
		<skos:definition>unit of energy widely used in nutrition</skos:definition>
		<fibo-fnd-utl-av:abbreviation>Cal</fibo-fnd-utl-av:abbreviation>
		<fibo-fnd-utl-av:abbreviation>kcal</fibo-fnd-utl-av:abbreviation>
		<fibo-fnd-utl-av:adaptedFrom rdf:datatype="&xsd;anyURI">https://en.wikipedia.org/wiki/Calorie</fibo-fnd-utl-av:adaptedFrom>
		<fibo-fnd-utl-av:explanatoryNote>The large calorie, food calorie, or kilocalorie (Cal, Calorie or kcal) is the amount of heat needed to cause the same increase in one kilogram of water (i.e., 4184 J). Thus, 1 kilocalorie (kcal) = 1000 calories (cal). By convention in food science, the large calorie is commonly called Calorie (with a capital C by some authors to distinguish from the smaller unit). In most countries, labels of industrialized food products are required to indicate the nutritional energy value in (kilo or large) calories per serving or per weight.</fibo-fnd-utl-av:explanatoryNote>
	</owl:NamedIndividual>
	
	<owl:Class rdf:about="&oe2020-pat-rec;Carbohydrate">
		<rdfs:subClassOf rdf:resource="&oe2020-pat-rec;Macronutrient"/>
		<rdfs:label>carbohydrate</rdfs:label>
		<skos:definition>any of various neutral compounds of carbon, hydrogen, and oxygen (as sugars, starches, and celluloses) most of which are formed by green plants and which constitute a major class of animal foods</skos:definition>
	</owl:Class>
	
	<owl:Class rdf:about="&oe2020-pat-rec;Cholesterol">
		<rdfs:subClassOf rdf:resource="&fibo-fnd-qt-qtu;QuantityValue"/>
		<rdfs:label>cholesterol</rdfs:label>
		<skos:definition>a sterol lipid synthesized by the liver and transported in the bloodstream to the membranes of all animal cells; it plays a central role in many biochemical processes and, as a lipoprotein that coats the walls of blood vessels, is associated with cardiovascular disease</skos:definition>
	</owl:Class>
	
	<owl:Class rdf:about="&oe2020-pat-rec;Cohort">
		<rdfs:subClassOf rdf:resource="&fibo-fnd-org-fm;Group"/>
		<rdfs:subClassOf rdf:resource="&fibo-fnd-utl-alx;StatisticalPopulation"/>
		<rdfs:subClassOf>
			<owl:Restriction>
				<owl:onProperty rdf:resource="&lcc-lr;hasMember"/>
				<owl:allValuesFrom rdf:resource="&fibo-fnd-aap-ppl;Person"/>
			</owl:Restriction>
		</rdfs:subClassOf>
		<rdfs:label>cohort</rdfs:label>
		<skos:definition>group of people that share a common characteristic</skos:definition>
		<fibo-fnd-utl-av:adaptedFrom rdf:datatype="&xsd;anyURI">https://dictionary.cambridge.org/us/dictionary/english/cohort</fibo-fnd-utl-av:adaptedFrom>
	</owl:Class>
	
	<owl:Class rdf:about="&oe2020-pat-rec;Condition">
		<rdfs:subClassOf rdf:resource="&fibo-fnd-pty-pty;Situation"/>
		<rdfs:label>condition</rdfs:label>
		<skos:definition>an abnormal state of health that interferes with the usual activities or feeling of wellbeing</skos:definition>
	</owl:Class>
	
	<owl:Class rdf:about="&oe2020-pat-rec;Culture">
		<rdfs:subClassOf rdf:resource="&oe2020-pat-rec;Lifestyle"/>
		<rdfs:label>culture</rdfs:label>
		<skos:definition>the conventional conducts and ideologies of a community; the system comprising of the accepted norms and values of a society</skos:definition>
	</owl:Class>
	
	<owl:Class rdf:about="&oe2020-pat-rec;Dairy">
		<rdfs:subClassOf rdf:resource="&oe2020-pat-rec;Food"/>
		<rdfs:label>dairy</rdfs:label>
		<owl:disjointWith rdf:resource="&oe2020-pat-rec;Fruit"/>
		<owl:disjointWith rdf:resource="&oe2020-pat-rec;Meat"/>
		<owl:disjointWith rdf:resource="&oe2020-pat-rec;Vegetable"/>
		<owl:disjointWith rdf:resource="&oe2020-pat-rec;WholeGrain"/>
		<skos:definition>food (such as ice cream, cheese, or yogurt) made primarily of or from milk</skos:definition>
	</owl:Class>
	
	<owl:NamedIndividual rdf:about="&oe2020-pat-rec;DeclinedToState">
		<rdf:type rdf:resource="&oe2020-pat-rec;GenderIdentity"/>
		<rdfs:label>declined to state</rdfs:label>
		<skos:definition>gender identity indicating that the individual chose not to provide information as of some date</skos:definition>
	</owl:NamedIndividual>
	
	<owl:Class rdf:about="&oe2020-pat-rec;Deficit">
		<rdfs:subClassOf rdf:resource="&oe2020-pat-rec;QualitativeMeasure"/>
		<rdfs:label>deficit</rdfs:label>
		<skos:definition>deficiency in amount or quality</skos:definition>
	</owl:Class>
	
	<owl:Class rdf:about="&oe2020-pat-rec;Demographic">
		<rdfs:subClassOf rdf:resource="&fibo-fnd-arr-cls;Classifier"/>
		<rdfs:subClassOf>
			<owl:Restriction>
				<owl:onProperty rdf:resource="&oe2020-pat-rec;canAffect"/>
				<owl:someValuesFrom rdf:resource="&oe2020-pat-rec;Lifestyle"/>
			</owl:Restriction>
		</rdfs:subClassOf>
		<rdfs:subClassOf>
			<owl:Restriction>
				<owl:onProperty rdf:resource="&oe2020-pat-rec;restricts"/>
				<owl:someValuesFrom rdf:resource="&oe2020-pat-rec;Guideline"/>
			</owl:Restriction>
		</rdfs:subClassOf>
		<rdfs:subClassOf>
			<owl:Restriction>
				<owl:onProperty rdf:resource="&lcc-cr;classifies"/>
				<owl:someValuesFrom rdf:resource="&oe2020-pat-rec;Cohort"/>
			</owl:Restriction>
		</rdfs:subClassOf>
		<rdfs:label>demographic</rdfs:label>
		<skos:definition>the statistical characteristics of human populations (such as age or income)</skos:definition>
	</owl:Class>
	
	<owl:Class rdf:about="&oe2020-pat-rec;Diabetes">
		<rdfs:subClassOf rdf:resource="&oe2020-pat-rec;Illness"/>
		<rdfs:label>diabetes</rdfs:label>
		<owl:disjointWith rdf:resource="&oe2020-pat-rec;Obesity"/>
		<skos:definition>a disease in which the body’s ability to produce or respond to the hormone insulin is impaired</skos:definition>
	</owl:Class>
	
	<owl:Class rdf:about="&oe2020-pat-rec;DiabeticPatientCohort">
		<rdfs:subClassOf rdf:resource="&fibo-fnd-pty-pty;Situation"/>
		<rdfs:subClassOf rdf:resource="&oe2020-pat-rec;Cohort"/>
		<rdfs:subClassOf>
			<owl:Restriction>
				<owl:onProperty rdf:resource="&fibo-fnd-pty-pty;hasActor"/>
				<owl:someValuesFrom rdf:resource="&oe2020-pat-rec;Patient"/>
			</owl:Restriction>
		</rdfs:subClassOf>
		<rdfs:subClassOf>
			<owl:Restriction>
				<owl:onProperty rdf:resource="&lcc-cr;isClassifiedBy"/>
				<owl:someValuesFrom rdf:resource="&oe2020-pat-rec;Demographic"/>
			</owl:Restriction>
		</rdfs:subClassOf>
		<rdfs:subClassOf>
			<owl:Restriction>
				<owl:onProperty rdf:resource="&lcc-cr;isClassifiedBy"/>
				<owl:someValuesFrom rdf:resource="&oe2020-pat-rec;Diabetes"/>
			</owl:Restriction>
		</rdfs:subClassOf>
		<rdfs:label>diabetic patient cohort</rdfs:label>
		<skos:definition>group of patients that have diabetes at some point in time</skos:definition>
	</owl:Class>
	
	<owl:Class rdf:about="&oe2020-pat-rec;Diet">
		<rdfs:subClassOf rdf:resource="&lcc-lr;Collection"/>
		<rdfs:subClassOf>
			<owl:Restriction>
				<owl:onProperty rdf:resource="&fibo-fnd-arr-arr;isConstituentOf"/>
				<owl:someValuesFrom rdf:resource="&oe2020-pat-rec;Lifestyle"/>
			</owl:Restriction>
		</rdfs:subClassOf>
		<rdfs:subClassOf>
			<owl:Restriction>
				<owl:onProperty rdf:resource="&fibo-fnd-rel-rel;comprises"/>
				<owl:someValuesFrom rdf:resource="&oe2020-pat-rec;Food"/>
			</owl:Restriction>
		</rdfs:subClassOf>
		<rdfs:subClassOf>
			<owl:Restriction>
				<owl:onProperty rdf:resource="&oe2020-pat-rec;restricts"/>
				<owl:someValuesFrom rdf:resource="&oe2020-pat-rec;Macronutrient"/>
			</owl:Restriction>
		</rdfs:subClassOf>
		<rdfs:label>diet</rdfs:label>
		<skos:definition>prescribed course of eating and drinking in which the amount and kind of food, as well as the times at which it is to be taken, are regulated for therapeutic purposes or selected with reference to a particular state of health</skos:definition>
		<fibo-fnd-utl-av:adaptedFrom>S. Chong, D. Ding, R. Byun, E. Comino, A. Bauman, and B. Jalaludin, &apos;Lifestyle Changes After a Diagnosis of Type 2 Diabetes,&apos; Diabetes spectrum : a publication of the American Diabetes Association, Feb-2017. [Online]. Available: https://www.ncbi.nlm.nih.gov/pmc/articles/PMC5309903/?fbclid=IwAR2dY5OKOjSBRXRGfKAQ4NQosTKp534nixdd8ac6KW55BT3SmFSTitGHbbY. [Accessed: 23-Sep-2020].</fibo-fnd-utl-av:adaptedFrom>
	</owl:Class>
	
	<owl:Class rdf:about="&oe2020-pat-rec;DietaryFat">
		<rdfs:subClassOf rdf:resource="&oe2020-pat-rec;Macronutrient"/>
		<rdfs:label>dietary fat</rdfs:label>
		<skos:definition>a macronutrient that provides energy for your body</skos:definition>
	</owl:Class>
	
	<owl:Class rdf:about="&oe2020-pat-rec;DietaryGoal">
		<rdfs:subClassOf rdf:resource="https://spec.edmcouncil.org/fibo/ontology/FND/GoalsAndObjectives/Objectives/Objective"/>
		<rdfs:label>dietary goal</rdfs:label>
		<skos:definition>a goal related to a diet</skos:definition>
	</owl:Class>
	
	<owl:Class rdf:about="&oe2020-pat-rec;Energy">
		<rdfs:label>energy</rdfs:label>
		<skos:definition>a quantity that denotes the ability to do work and is measured in a unit dimensioned in mass × distance²/time² (ML²/T²) or the equivalent</skos:definition>
	</owl:Class>
	
	<owl:Class rdf:about="&oe2020-pat-rec;EnergyDeficit">
		<rdfs:subClassOf rdf:resource="&oe2020-pat-rec;Deficit"/>
		<rdfs:label>energy deficit</rdfs:label>
		<skos:definition>a deficit related to energy</skos:definition>
	</owl:Class>
	
	<owl:Class rdf:about="&oe2020-pat-rec;EnergySurplus">
		<rdfs:subClassOf rdf:resource="&oe2020-pat-rec;Surplus"/>
		<rdfs:label>energy surplus</rdfs:label>
		<skos:definition>a surplus related to energy</skos:definition>
	</owl:Class>
	
	<owl:Class rdf:about="&oe2020-pat-rec;EvidenceOfDisease">
		<rdfs:subClassOf rdf:resource="&oe2020-pat-rec;Condition"/>
		<rdfs:label>evidence of disease</rdfs:label>
		<skos:definition>any objective sign that the disease exists in the body, as opposed to a symptom, which is, by nature, subjective</skos:definition>
	</owl:Class>
	
	<owl:Class rdf:about="&oe2020-pat-rec;Exercise">
		<rdfs:subClassOf>
			<owl:Restriction>
				<owl:onProperty rdf:resource="&fibo-fnd-arr-arr;isConstituentOf"/>
				<owl:someValuesFrom rdf:resource="&oe2020-pat-rec;Lifestyle"/>
			</owl:Restriction>
		</rdfs:subClassOf>
		<rdfs:label>exercise</rdfs:label>
		<skos:definition>bodily exertion for the sake of developing and maintaining physical fitness</skos:definition>
	</owl:Class>
	
	<owl:NamedIndividual rdf:about="&oe2020-pat-rec;Female">
		<rdf:type rdf:resource="&oe2020-pat-rec;GenderIdentity"/>
		<rdf:type rdf:resource="&oe2020-pat-rec;SexAssignedAtBirth"/>
		<rdfs:label>female</rdfs:label>
		<skos:definition>belonging to the sex which typically produces eggs (ova), or to the gender which is typically associated with it</skos:definition>
	</owl:NamedIndividual>
	
	<owl:NamedIndividual rdf:about="&oe2020-pat-rec;FemaleGroup">
		<rdf:type rdf:resource="&oe2020-pat-rec;GenderIdentityGroup"/>
		<rdfs:label>female group</rdfs:label>
		<skos:definition>gender identity group including individuals that self-identify as female</skos:definition>
	</owl:NamedIndividual>
	
	<owl:Class rdf:about="&oe2020-pat-rec;Fiber">
		<rdfs:subClassOf rdf:resource="&oe2020-pat-rec;Macronutrient"/>
		<rdfs:label>fiber</rdfs:label>
		<skos:definition>material in food that stimulates the intestine and promotes elimination of waste from the large intestine</skos:definition>
	</owl:Class>
	
	<owl:Class rdf:about="&oe2020-pat-rec;Food">
		<rdfs:subClassOf rdf:resource="&fibo-fnd-pas-pas;Product"/>
		<rdfs:subClassOf>
			<owl:Restriction>
				<owl:onProperty rdf:resource="&oe2020-pat-rec;contains"/>
				<owl:someValuesFrom rdf:resource="&oe2020-pat-rec;Macronutrient"/>
			</owl:Restriction>
		</rdfs:subClassOf>
		<rdfs:label>food</rdfs:label>
		<skos:definition>material consisting essentially of protein, carbohydrate, and fat used in the body of an organism to sustain growth, repair, and vital processes and to furnish energy</skos:definition>
		<fibo-fnd-utl-av:adaptedFrom rdf:datatype="&xsd;anyURI">https://www.merriam-webster.com/dictionary/food</fibo-fnd-utl-av:adaptedFrom>
	</owl:Class>
	
	<owl:Class rdf:about="&oe2020-pat-rec;Fruit">
		<rdfs:subClassOf rdf:resource="&oe2020-pat-rec;Food"/>
		<rdfs:label>fruit</rdfs:label>
		<owl:disjointWith rdf:resource="&oe2020-pat-rec;Meat"/>
		<owl:disjointWith rdf:resource="&oe2020-pat-rec;Vegetable"/>
		<owl:disjointWith rdf:resource="&oe2020-pat-rec;WholeGrain"/>
		<skos:definition>the usually edible reproductive body of a seed plant, especially one having a sweet pulp associated with the seed</skos:definition>
	</owl:Class>
	
	<owl:Class rdf:about="&oe2020-pat-rec;GenderIdentity">
		<rdfs:subClassOf rdf:resource="&fibo-fnd-arr-cls;Classifier"/>
		<rdfs:subClassOf>
			<owl:Restriction>
				<owl:onProperty rdf:resource="&fibo-fnd-dt-fd;hasAsOfDate"/>
				<owl:onClass rdf:resource="&fibo-fnd-dt-fd;ExplicitDate"/>
				<owl:qualifiedCardinality rdf:datatype="&xsd;nonNegativeInteger">1</owl:qualifiedCardinality>
			</owl:Restriction>
		</rdfs:subClassOf>
		<rdfs:label>gender identity</rdfs:label>
		<skos:definition>classifier indicating one&apos;s personal experience of one&apos;s own gender</skos:definition>
	</owl:Class>
	
	<owl:Class rdf:about="&oe2020-pat-rec;GenderIdentityGroup">
		<rdfs:subClassOf rdf:resource="&oe2020-pat-rec;Demographic"/>
		<rdfs:label>gender identity group</rdfs:label>
		<skos:definition>demographic indicating a qualitative value for gender identity that a member of a population identifies with at some point in time</skos:definition>
	</owl:Class>
	
	<owl:Class rdf:about="&oe2020-pat-rec;Guideline">
		<rdfs:subClassOf>
			<owl:Restriction>
				<owl:onProperty rdf:resource="&oe2020-pat-rec;recommends"/>
				<owl:someValuesFrom rdf:resource="&oe2020-pat-rec;Exercise"/>
			</owl:Restriction>
		</rdfs:subClassOf>
		<rdfs:subClassOf>
			<owl:Restriction>
				<owl:onProperty rdf:resource="&oe2020-pat-rec;recommends"/>
				<owl:someValuesFrom rdf:resource="&oe2020-pat-rec;Lifestyle"/>
			</owl:Restriction>
		</rdfs:subClassOf>
		<rdfs:label>guideline</rdfs:label>
		<skos:definition>a general rule, principle, or piece of advice</skos:definition>
	</owl:Class>
	
	<owl:Class rdf:about="&oe2020-pat-rec;Illness">
		<rdfs:subClassOf>
			<owl:Restriction>
				<owl:onProperty rdf:resource="&oe2020-pat-rec;isTreatedWith"/>
				<owl:someValuesFrom rdf:resource="&oe2020-pat-rec;Medicine"/>
			</owl:Restriction>
		</rdfs:subClassOf>
		<rdfs:label>illness</rdfs:label>
		<skos:definition>an unhealthy condition of body or mind</skos:definition>
	</owl:Class>
	
	<owl:Class rdf:about="&oe2020-pat-rec;Insulin">
		<rdfs:subClassOf rdf:resource="&oe2020-pat-rec;Medicine"/>
		<rdfs:label>insulin</rdfs:label>
		<skos:definition>a hormone that is essential for the metabolism of carbohydrates and the regulation of glucose levels in the blood</skos:definition>
	</owl:Class>
	
	<owl:Class rdf:about="&oe2020-pat-rec;Jogging">
		<rdfs:subClassOf rdf:resource="&oe2020-pat-rec;Exercise"/>
		<rdfs:label>jogging</rdfs:label>
		<skos:definition>to run or ride at a slow trot</skos:definition>
	</owl:Class>
	
	<owl:Class rdf:about="&oe2020-pat-rec;Legume">
		<rdfs:subClassOf rdf:resource="&oe2020-pat-rec;Food"/>
		<rdfs:label>legume</rdfs:label>
		<skos:definition>the fruit or seed of plants of the legume family (such as peas or beans) used for food</skos:definition>
	</owl:Class>
	
	<owl:Class rdf:about="&oe2020-pat-rec;Lifestyle">
		<rdfs:subClassOf rdf:resource="&fibo-fnd-arr-cls;Classifier"/>
		<rdfs:label>lifestyle</rdfs:label>
		<skos:definition>the typical way of life of an individual, group, or culture</skos:definition>
	</owl:Class>
	
	<owl:Class rdf:about="&oe2020-pat-rec;Macronutrient">
		<rdfs:label>macronutrient</rdfs:label>
		<skos:definition>a chemical element or substance (such as potassium or protein) that is essential in relatively large amounts to the growth and health of a living organism</skos:definition>
	</owl:Class>
	
	<owl:NamedIndividual rdf:about="&oe2020-pat-rec;Male">
		<rdf:type rdf:resource="&oe2020-pat-rec;GenderIdentity"/>
		<rdf:type rdf:resource="&oe2020-pat-rec;SexAssignedAtBirth"/>
		<rdfs:label>male</rdfs:label>
		<skos:definition>of, relating to, or being the sex that typically has the capacity to produce relatively small, usually motile gametes which fertilize the eggs of a female</skos:definition>
	</owl:NamedIndividual>
	
	<owl:NamedIndividual rdf:about="&oe2020-pat-rec;MaleGroup">
		<rdf:type rdf:resource="&oe2020-pat-rec;GenderIdentityGroup"/>
		<rdfs:label>male group</rdfs:label>
		<skos:definition>gender identity group including individuals that self-identify as male</skos:definition>
	</owl:NamedIndividual>
	
	<owl:Class rdf:about="&oe2020-pat-rec;Meat">
		<rdfs:subClassOf rdf:resource="&oe2020-pat-rec;Food"/>
		<rdfs:label>meat</rdfs:label>
		<owl:disjointWith rdf:resource="&oe2020-pat-rec;Vegetable"/>
		<owl:disjointWith rdf:resource="&oe2020-pat-rec;WholeGrain"/>
		<skos:definition>animal tissue considered especially as food</skos:definition>
	</owl:Class>
	
	<owl:Class rdf:about="&oe2020-pat-rec;Medicine">
		<rdfs:label>medicine</rdfs:label>
		<skos:definition>a compound or preparation used for the treatment or prevention of disease, especially a drug or drugs taken by mouth</skos:definition>
	</owl:Class>
	
	<owl:NamedIndividual rdf:about="&oe2020-pat-rec;NonBinary">
		<rdf:type rdf:resource="&oe2020-pat-rec;GenderIdentity"/>
		<rdfs:label>non-binary</rdfs:label>
		<skos:definition>gender identity indicating that the individual self-identifies as not being exclusively masculine or feminine, i.e., as being outside of the gender binary</skos:definition>
	</owl:NamedIndividual>
	
	<owl:NamedIndividual rdf:about="&oe2020-pat-rec;NonBinaryGroup">
		<rdf:type rdf:resource="&oe2020-pat-rec;GenderIdentityGroup"/>
		<rdfs:label>non-binary group</rdfs:label>
		<skos:definition>gender identity group including individuals that self-identify as not being exclusively masculine or feminine, i.e., as being outside of the gender binary</skos:definition>
	</owl:NamedIndividual>
	
	<owl:NamedIndividual rdf:about="&oe2020-pat-rec;None">
		<rdf:type rdf:resource="&oe2020-pat-rec;GenderIdentityGroup"/>
		<rdfs:label>none</rdfs:label>
		<skos:definition>gender identity group including individuals that do not self-identify as belonging to any defined group</skos:definition>
	</owl:NamedIndividual>
	
	<owl:Class rdf:about="&oe2020-pat-rec;Obesity">
		<rdfs:subClassOf rdf:resource="&oe2020-pat-rec;Illness"/>
		<rdfs:subClassOf>
			<owl:Restriction>
				<owl:onProperty rdf:resource="&oe2020-pat-rec;canIncrease"/>
				<owl:someValuesFrom rdf:resource="&oe2020-pat-rec;Cholesterol"/>
			</owl:Restriction>
		</rdfs:subClassOf>
		<rdfs:subClassOf>
			<owl:Restriction>
				<owl:onProperty rdf:resource="&oe2020-pat-rec;indicates"/>
				<owl:someValuesFrom rdf:resource="&oe2020-pat-rec;Type2Diabetes"/>
			</owl:Restriction>
		</rdfs:subClassOf>
		<rdfs:label>obesity</rdfs:label>
		<skos:definition>the condition of being grossly fat or overweight</skos:definition>
	</owl:Class>
	
	<owl:Class rdf:about="&oe2020-pat-rec;Patient">
		<rdfs:subClassOf rdf:resource="&fibo-fnd-pty-pty;Actor"/>
		<rdfs:subClassOf>
			<owl:Restriction>
				<owl:onProperty rdf:resource="&fibo-fnd-pty-rl;isPlayedBy"/>
				<owl:onClass rdf:resource="&fibo-fnd-aap-ppl;Person"/>
				<owl:qualifiedCardinality rdf:datatype="&xsd;nonNegativeInteger">1</owl:qualifiedCardinality>
			</owl:Restriction>
		</rdfs:subClassOf>
		<rdfs:label>patient</rdfs:label>
		<skos:definition>person who receives medical attention, care, or treatment, or who is registered with medical professional or institution with the purpose to receive medical care when necessary</skos:definition>
	</owl:Class>
	
	<owl:Class rdf:about="&oe2020-pat-rec;PersonAge">
		<rdfs:subClassOf rdf:resource="&oe2020-pat-rec;Age"/>
		<rdfs:subClassOf>
			<owl:Restriction>
				<owl:onProperty rdf:resource="&oe2020-pat-rec;isCalculatedFromBirth"/>
				<owl:onClass rdf:resource="&fibo-fnd-aap-ppl;DateOfBirth"/>
				<owl:qualifiedCardinality rdf:datatype="&xsd;nonNegativeInteger">1</owl:qualifiedCardinality>
			</owl:Restriction>
		</rdfs:subClassOf>
		<rdfs:subClassOf>
			<owl:Restriction>
				<owl:onProperty rdf:resource="&fibo-fnd-dt-fd;hasAsOfDate"/>
				<owl:onClass rdf:resource="&fibo-fnd-dt-fd;ExplicitDate"/>
				<owl:qualifiedCardinality rdf:datatype="&xsd;nonNegativeInteger">1</owl:qualifiedCardinality>
			</owl:Restriction>
		</rdfs:subClassOf>
		<rdfs:label>person age</rdfs:label>
		<skos:definition>period of time a person has been alive</skos:definition>
		<fibo-fnd-utl-av:adaptedFrom rdf:datatype="&xsd;anyURI">https://dictionary.cambridge.org/dictionary/english/age</fibo-fnd-utl-av:adaptedFrom>
	</owl:Class>
	
	<owl:Class rdf:about="&oe2020-pat-rec;Protein">
		<rdfs:subClassOf rdf:resource="&oe2020-pat-rec;Macronutrient"/>
		<rdfs:label>protein</rdfs:label>
		<skos:definition>a nutrient found in food (as meat, milk, eggs, and beans) that is made up of many amino acids joined together, is a necessary part of the diet, and is essential for normal cell structure and function</skos:definition>
	</owl:Class>
	
	<owl:Class rdf:about="&oe2020-pat-rec;QualitativeMeasure">
		<rdfs:subClassOf rdf:resource="&fibo-fnd-utl-alx;Measure"/>
		<rdfs:label>qualitative measure</rdfs:label>
		<skos:definition>relating to, measuring, or measured by the quality of something rather than its quantity</skos:definition>
	</owl:Class>
	
	<owl:Class rdf:about="&oe2020-pat-rec;Sedentary">
		<rdfs:subClassOf rdf:resource="&oe2020-pat-rec;ActivityLevel"/>
		<rdfs:label>sedentary</rdfs:label>
		<skos:definition>not physically active</skos:definition>
	</owl:Class>
	
	<owl:Class rdf:about="&oe2020-pat-rec;SedentaryBehavior">
		<rdfs:subClassOf rdf:resource="&oe2020-pat-rec;Lifestyle"/>
		<rdfs:label>sedentary behavior</rdfs:label>
		<skos:definition>a type of lifestyle that lacks physical exercise, characterized by sitting, reading, watching television or using a computer for much of the day without vigorous physical exertion</skos:definition>
	</owl:Class>
	
	<owl:Class rdf:about="&oe2020-pat-rec;SemiActive">
		<rdfs:subClassOf rdf:resource="&oe2020-pat-rec;ActivityLevel"/>
		<rdfs:label>semi active</rdfs:label>
		<skos:definition>somewhere between active and sedentary</skos:definition>
	</owl:Class>
	
	<owl:Class rdf:about="&oe2020-pat-rec;Serving">
		<rdfs:subClassOf rdf:resource="&fibo-fnd-qt-qtu;Quantity"/>
		<rdfs:label>serving</rdfs:label>
		<skos:definition>a quantity of food suitable for or served to one person</skos:definition>
	</owl:Class>
	
	<owl:Class rdf:about="&oe2020-pat-rec;SexAssignedAtBirth">
		<rdfs:subClassOf rdf:resource="&fibo-fnd-arr-cls;Classifier"/>
		<rdfs:label>sex assigned at birth</rdfs:label>
		<skos:definition>the discernment of an infant&apos;s sex at birth, which usually aligns with a child&apos;s anatomical sex and phenotype</skos:definition>
	</owl:Class>
	
	<owl:Class rdf:about="&oe2020-pat-rec;Surplus">
		<rdfs:subClassOf rdf:resource="&oe2020-pat-rec;QualitativeMeasure"/>
		<rdfs:label>surplus</rdfs:label>
		<skos:definition>excess in amount or quality</skos:definition>
	</owl:Class>
	
	<owl:Class rdf:about="&oe2020-pat-rec;TransFat">
		<rdfs:subClassOf rdf:resource="&oe2020-pat-rec;Macronutrient"/>
		<rdfs:label>trans fat</rdfs:label>
		<skos:definition>a fat containing trans-fatty acids</skos:definition>
	</owl:Class>
	
	<owl:NamedIndividual rdf:about="&oe2020-pat-rec;Transgender">
		<rdf:type rdf:resource="&oe2020-pat-rec;GenderIdentity"/>
		<rdfs:label>transgender</rdfs:label>
		<skos:definition>gender identity indicating that the individual self-identifies as having a gender identity or gender expression that differs with their assigned sex at birth</skos:definition>
	</owl:NamedIndividual>
	
	<owl:NamedIndividual rdf:about="&oe2020-pat-rec;TransgenderGroup">
		<rdf:type rdf:resource="&oe2020-pat-rec;GenderIdentityGroup"/>
		<rdfs:label>transgender group</rdfs:label>
		<skos:definition>gender identity including individuals that self-identify as having a gender identity or gender expression that differs with their assigned sex at birth</skos:definition>
	</owl:NamedIndividual>
	
	<owl:Class rdf:about="&oe2020-pat-rec;Type2Diabetes">
		<rdfs:subClassOf rdf:resource="&oe2020-pat-rec;Diabetes"/>
		<rdfs:label>type 2 diabetes</rdfs:label>
		<skos:definition>a type of diabetes mellitus that is characterized by insulin resistance or desensitization and increased blood glucose levels</skos:definition>
	</owl:Class>
	
	<owl:Class rdf:about="&oe2020-pat-rec;Vegetable">
		<rdfs:subClassOf rdf:resource="&oe2020-pat-rec;Food"/>
		<rdfs:label>vegetable</rdfs:label>
		<owl:disjointWith rdf:resource="&oe2020-pat-rec;WholeGrain"/>
		<skos:definition>a usually herbaceous plant (such as the cabbage, bean, or potato) grown for an edible part that is usually eaten as part of a meal</skos:definition>
	</owl:Class>
	
	<owl:Class rdf:about="&oe2020-pat-rec;WholeGrain">
		<rdfs:subClassOf rdf:resource="&oe2020-pat-rec;Food"/>
		<rdfs:label>whole grain</rdfs:label>
		<skos:definition>a cereal grain that contains cereal germ, endosperm, and bran, in contrast to refined grains, which retain only the endosperm</skos:definition>
	</owl:Class>
	
	<owl:Class rdf:about="&oe2020-pat-rec;Yoga">
		<rdfs:subClassOf rdf:resource="&oe2020-pat-rec;Exercise"/>
		<rdfs:label>yoga</rdfs:label>
		<skos:definition>a system of physical postures, breathing techniques, and sometimes meditation derived from Yoga but often practiced independently especially in Western cultures to promote physical and emotional well-being</skos:definition>
	</owl:Class>
	
	<owl:ObjectProperty rdf:about="&oe2020-pat-rec;benefits">
		<rdfs:label>benefits</rdfs:label>
		<skos:definition>something that produces good or helpful results or effects or that promotes well-being</skos:definition>
	</owl:ObjectProperty>
	
	<owl:ObjectProperty rdf:about="&oe2020-pat-rec;canAffect">
		<rdfs:label>can affect</rdfs:label>
		<skos:editorialNote>to produce an effect upon someone or something</skos:editorialNote>
	</owl:ObjectProperty>
	
	<owl:ObjectProperty rdf:about="&oe2020-pat-rec;canIncrease">
		<rdfs:label>can increase</rdfs:label>
		<skos:definition>to become progressively greater</skos:definition>
	</owl:ObjectProperty>
	
	<owl:ObjectProperty rdf:about="&oe2020-pat-rec;contains">
		<rdf:type rdf:resource="&owl;TransitiveProperty"/>
		<rdfs:label>contains</rdfs:label>
		<skos:definition>to have within</skos:definition>
	</owl:ObjectProperty>
	
	<owl:ObjectProperty rdf:about="&oe2020-pat-rec;decreases">
		<rdfs:label>decreases</rdfs:label>
		<skos:definition>to grow progressively less (as in size, amount, number, or intensity)</skos:definition>
	</owl:ObjectProperty>
	
	<owl:ObjectProperty rdf:about="&oe2020-pat-rec;eats">
		<rdfs:label>eats</rdfs:label>
		<skos:definition>put (food) into the mouth and chew and swallow it.</skos:definition>
	</owl:ObjectProperty>
	
	<owl:ObjectProperty rdf:about="&oe2020-pat-rec;engagesIn">
		<rdfs:label>engages in</rdfs:label>
		<skos:definition>to induce to participate</skos:definition>
	</owl:ObjectProperty>
	
	<owl:ObjectProperty rdf:about="&oe2020-pat-rec;harms">
		<rdfs:label>harms</rdfs:label>
		<skos:definition>physical or mental damage</skos:definition>
	</owl:ObjectProperty>
	
	<owl:ObjectProperty rdf:about="&oe2020-pat-rec;hasAge">
		<rdfs:subPropertyOf rdf:resource="&fibo-fnd-rel-rel;isCharacterizedBy"/>
		<rdfs:label>has age</rdfs:label>
		<rdfs:range rdf:resource="&oe2020-pat-rec;Age"/>
		<skos:definition>indicates the length of time someone has been alive or something has existed</skos:definition>
	</owl:ObjectProperty>
	
	<owl:ObjectProperty rdf:about="&oe2020-pat-rec;hasCharacteristic">
		<rdfs:label>has characteristic</rdfs:label>
		<skos:definition>a distinguishing trait, quality, or property</skos:definition>
	</owl:ObjectProperty>
	
	<owl:ObjectProperty rdf:about="&oe2020-pat-rec;hasGenderIdentity">
		<rdfs:subPropertyOf rdf:resource="&fibo-fnd-rel-rel;isCharacterizedBy"/>
		<rdfs:label>has gender identity</rdfs:label>
		<rdfs:range rdf:resource="&oe2020-pat-rec;GenderIdentity"/>
		<skos:definition>indicates the gender as reported by an individual</skos:definition>
	</owl:ObjectProperty>
	
	<owl:ObjectProperty rdf:about="&oe2020-pat-rec;increases">
		<rdfs:label>increases</rdfs:label>
		<skos:definition>to become progressively greater (as in size, amount, number, or intensity)</skos:definition>
	</owl:ObjectProperty>
	
	<owl:ObjectProperty rdf:about="&oe2020-pat-rec;indicates">
	</owl:ObjectProperty>
	
	<owl:ObjectProperty rdf:about="&oe2020-pat-rec;isAfflictedWith">
		<rdfs:label>is afflicted with</rdfs:label>
		<skos:definition>grievously affected or troubled</skos:definition>
	</owl:ObjectProperty>
	
	<owl:ObjectProperty rdf:about="&oe2020-pat-rec;isCalculatedFromBirth">
		<rdfs:subPropertyOf rdf:resource="&fibo-fnd-dt-fd;hasStartDate"/>
		<rdfs:label>is calculated from birth</rdfs:label>
		<rdfs:range rdf:resource="&fibo-fnd-aap-ppl;DateOfBirth"/>
		<skos:definition>indicates the date from which age is calculated</skos:definition>
		<fibo-fnd-utl-av:adaptedFrom rdf:datatype="&xsd;anyURI">https://dictionary.cambridge.org/dictionary/english/age</fibo-fnd-utl-av:adaptedFrom>
	</owl:ObjectProperty>
	
	<owl:ObjectProperty rdf:about="&oe2020-pat-rec;isRiskFactorFor">
		<rdf:type rdf:resource="&owl;TransitiveProperty"/>
		<rdfs:label>is risk factor for</rdfs:label>
		<skos:definition>something that increases risk or susceptibility</skos:definition>
	</owl:ObjectProperty>
	
	<owl:ObjectProperty rdf:about="&oe2020-pat-rec;isTreatedWith">
		<rdfs:label>is treated with</rdfs:label>
		<skos:definition>to care for or deal with medically or surgically</skos:definition>
	</owl:ObjectProperty>
	
	<owl:ObjectProperty rdf:about="&oe2020-pat-rec;livesWith">
		<rdfs:label>lives with</rdfs:label>
		<skos:definition>to dwell with</skos:definition>
	</owl:ObjectProperty>
	
	<owl:ObjectProperty rdf:about="&oe2020-pat-rec;recommends">
		<rdfs:label>recommends</rdfs:label>
		<skos:definition>to suggest an act or course of action</skos:definition>
	</owl:ObjectProperty>
	
	<owl:ObjectProperty rdf:about="&oe2020-pat-rec;restricts">
		<rdfs:label>restricts</rdfs:label>
		<rdfs:domain>
			<owl:Class>
				<owl:unionOf rdf:parseType="Collection">
					<rdf:Description rdf:about="&oe2020-pat-rec;Diet">
					</rdf:Description>
					<rdf:Description rdf:about="&oe2020-pat-rec;Guideline">
					</rdf:Description>
				</owl:unionOf>
			</owl:Class>
		</rdfs:domain>
		<skos:definition>to confine within bounds</skos:definition>
	</owl:ObjectProperty>
	
	<owl:ObjectProperty rdf:about="&lcc-cr;isClassifiedBy">
	</owl:ObjectProperty>
	
	<owl:AllDisjointClasses>
		<owl:members rdf:parseType="Collection">
			<rdf:Description rdf:about="&oe2020-pat-rec;Active">
			</rdf:Description>
			<rdf:Description rdf:about="&oe2020-pat-rec;Sedentary">
			</rdf:Description>
			<rdf:Description rdf:about="&oe2020-pat-rec;SemiActive">
			</rdf:Description>
		</owl:members>
	</owl:AllDisjointClasses>
	<owl:AllDisjointClasses>
		<owl:members rdf:parseType="Collection">
			<rdf:Description rdf:about="&oe2020-pat-rec;AerobicExercise">
			</rdf:Description>
			<rdf:Description rdf:about="&oe2020-pat-rec;BodyWeightExercise">
			</rdf:Description>
			<rdf:Description rdf:about="&oe2020-pat-rec;Jogging">
			</rdf:Description>
			<rdf:Description rdf:about="&oe2020-pat-rec;Yoga">
			</rdf:Description>
		</owl:members>
	</owl:AllDisjointClasses>
	<owl:AllDisjointClasses>
		<owl:members rdf:parseType="Collection">
			<rdf:Description rdf:about="&oe2020-pat-rec;Dairy">
			</rdf:Description>
			<rdf:Description rdf:about="&oe2020-pat-rec;Fruit">
			</rdf:Description>
			<rdf:Description rdf:about="&oe2020-pat-rec;Legume">
			</rdf:Description>
			<rdf:Description rdf:about="&oe2020-pat-rec;Meat">
			</rdf:Description>
			<rdf:Description rdf:about="&oe2020-pat-rec;Vegetable">
			</rdf:Description>
			<rdf:Description rdf:about="&oe2020-pat-rec;WholeGrain">
			</rdf:Description>
		</owl:members>
	</owl:AllDisjointClasses>
</rdf:RDF>
