# baseURI: https://tw.rpi.edu/ontology-engineering/oe2022/indoor-environment-manager/n# imports: https://www.omg.org/spec/Commons/AnnotationVocabulary/n# imports: https://www.omg.org/spec/Commons/Classifiers/n# imports: https://www.omg.org/spec/Commons/Collections/n# imports: https://www.omg.org/spec/Commons/DatesAndTimes/n# imports: https://www.omg.org/spec/Commons/Designators/n# imports: https://www.omg.org/spec/Commons/PartiesAndSituations/n# imports: https://www.omg.org/spec/Commons/QuantitiesAndUnits/nn@base <https://tw.rpi.edu/ontology-engineering/oe2022/indoor-environment-manager/> .n@prefix : <https://tw.rpi.edu/ontology-engineering/oe2022/indoor-environment-manager/> .n@prefix cmns-av: <https://www.omg.org/spec/Commons/AnnotationVocabulary/> .n@prefix cmns-cls: <https://www.omg.org/spec/Commons/Classifiers/> .n@prefix cmns-col: <https://www.omg.org/spec/Commons/Collections/> .n@prefix cmns-dsg: <https://www.omg.org/spec/Commons/Designators/> .n@prefix cmns-dt: <https://www.omg.org/spec/Commons/DatesAndTimes/> .n@prefix cmns-pts: <https://www.omg.org/spec/Commons/PartiesAndSituations/> .n@prefix cmns-qtu: <https://www.omg.org/spec/Commons/QuantitiesAndUnits/> .n@prefix dct: <http://purl.org/dc/terms/> .n@prefix oe2022-iem: <https://tw.rpi.edu/ontology-engineering/oe2022/indoor-environment-manager/> .n@prefix owl: <http://www.w3.org/2002/07/owl#> .n@prefix rdf: <http://www.w3.org/1999/02/22-rdf-syntax-ns#> .n@prefix rdfs: <http://www.w3.org/2000/01/rdf-schema#> .n@prefix skos: <http://www.w3.org/2004/02/skos/core#> .n@prefix xsd: <http://www.w3.org/2001/XMLSchema#> .nn<https://tw.rpi.edu/ontology-engineering/oe2022/indoor-environment-manager/>n	a owl:Ontology ;n	rdfs:label "Indoor Environment Manager Ontology" ;n	dct:abstract "" ;n	owl:importsn		<https://www.omg.org/spec/Commons/AnnotationVocabulary/> ,n		<https://www.omg.org/spec/Commons/Classifiers/> ,n		<https://www.omg.org/spec/Commons/Collections/> ,n		<https://www.omg.org/spec/Commons/DatesAndTimes/> ,n		<https://www.omg.org/spec/Commons/Designators/> ,n		<https://www.omg.org/spec/Commons/PartiesAndSituations/> ,n		<https://www.omg.org/spec/Commons/QuantitiesAndUnits/>n		;n	.nnoe2022-iem:AirQualityn	an		owl:NamedIndividual ,n		owl:Class ,n		cmns-qtu:QuantityKindn		;n	rdfs:subClassOf oe2022-iem:IndoorEnvironmentalQuality ;n	rdfs:label "air quality" ;n	owl:disjointWith oe2022-iem:ThermalComfort ;n	skos:definition "Synthesis of various physical measurements of properties of air that threaten human health" ;n	cmns-qtu:hasMeasurementUnit oe2022-iem:AirQualityIndex ;n	.nnoe2022-iem:AirQualityIndexn	an		owl:NamedIndividual ,n		cmns-qtu:ArbitraryUnitn		;n	rdfs:label "air quality index" ;n	skos:definition "measurement that combines other meaurements of properties of air to indicate the level of danger to human health" ;n	.nnoe2022-iem:ClosedStaten	a owl:Class ;n	rdfs:subClassOf oe2022-iem:ComponentState ;n	rdfs:label "closed state" ;n	owl:disjointWith oe2022-iem:ThermostatState ;n	skos:definition "condition of being not open" ;n	.nnoe2022-iem:ComponentStaten	a owl:Class ;n	rdfs:label "component state" ;n	skos:definition "an object in a room that can be used to alter relevant IEQ parameters" ;n	.nnoe2022-iem:Costn	an		owl:NamedIndividual ,n		cmns-qtu:BaseQuantityKindn		;n	rdfs:label "cost" ;n	skos:definition "amount paid or charged for something" ;n	.nnoe2022-iem:Dehumidifiern	a owl:Class ;n	rdfs:subClassOfn		oe2022-iem:Equipment ,n		[n			a owl:Restriction ;n			owl:onProperty oe2022-iem:hasState ;n			owl:allValuesFrom [n				a owl:Class ;n				owl:unionOf (n					oe2022-iem:OffStaten					oe2022-iem:OnStaten				) ;n			] ;n		]n		;n	rdfs:label "dehumidifier" ;n	skos:definition "room component that can be on or off, thereby lowering indoor relative humidity or not, respectively" ;n	.nnoe2022-iem:Energyn	an		owl:NamedIndividual ,n		cmns-qtu:BaseQuantityKindn		;n	rdfs:label "energy" ;n	skos:definition "measurement of the ability of something to do work" ;n	.nnoe2022-iem:EnergyUsagen	a owl:Class ;n	rdfs:subClassOf [n		a owl:Restriction ;n		owl:onProperty cmns-qtu:hasQuantityValue ;n		owl:someValuesFrom [n			a owl:Class ;n			owl:intersectionOf (n				cmns-qtu:QuantityValuen				[n					a owl:Restriction ;n					owl:onProperty cmns-qtu:hasMeasurementUnit ;n					owl:someValuesFrom [n						a owl:Restriction ;n						owl:onProperty cmns-qtu:hasQuantityKind ;n						owl:hasValue oe2022-iem:Energy ;n					] ;n				]n			) ;n		] ;n	] ;n	rdfs:label "energy usage" ;n	skos:definition "quantity of energy used to power some equipment, per unit time" ;n	.nnoe2022-iem:EnvironmentAttributen	a owl:Class ;n	rdfs:label "environment attribute" ;n	skos:definition "a quantitative attribute of local environment" ;n	.nnoe2022-iem:Equipmentn	a owl:Class ;n	rdfs:subClassOfn		oe2022-iem:RoomComponent ,n		[n			a owl:Restriction ;n			owl:onProperty oe2022-iem:hasState ;n			owl:onClass oe2022-iem:ComponentState ;n			owl:qualifiedCardinality "1"^^xsd:nonNegativeInteger ;n		] ,n		[n			a owl:Restriction ;n			owl:onProperty oe2022-iem:hasAttribute ;n			owl:onClass oe2022-iem:EnergyUsage ;n			owl:qualifiedCardinality "1"^^xsd:nonNegativeInteger ;n		]n		;n	rdfs:label "equipment" ;n	owl:disjointWith oe2022-iem:Furniture ;n	skos:definition "room component that consumes energy" ;n	.nnoe2022-iem:EquipmentEnergyUsagen	a owl:Class ;n	rdfs:label "equipment energy usage" ;n	skos:definition "Energy consumption used by equipment in a room" ;n	.nnoe2022-iem:Fann	a owl:Class ;n	rdfs:subClassOfn		oe2022-iem:Equipment ,n		[n			a owl:Restriction ;n			owl:onProperty oe2022-iem:hasState ;n			owl:allValuesFrom [n				a owl:Class ;n				owl:unionOf (n					oe2022-iem:OffStaten					oe2022-iem:OnStaten				) ;n			] ;n		]n		;n	rdfs:label "fan" ;n	skos:definition "HVAC equipment that can increase air speed" ;n	.nnoe2022-iem:Furnituren	a owl:Class ;n	rdfs:subClassOfn		oe2022-iem:RoomComponent ,n		[n			a owl:Restriction ;n			owl:onProperty oe2022-iem:hasState ;n			owl:allValuesFrom [n				a owl:Class ;n				owl:unionOf (n					oe2022-iem:ClosedStaten					oe2022-iem:OpenStaten				) ;n			] ;n		] ,n		[n			a owl:Restriction ;n			owl:onProperty oe2022-iem:hasState ;n			owl:onClass oe2022-iem:ComponentState ;n			owl:qualifiedCardinality "1"^^xsd:nonNegativeInteger ;n		]n		;n	rdfs:label "furniture" ;n	skos:definition "room component that does not consume energy" ;n	.nnoe2022-iem:Gramn	an		owl:NamedIndividual ,n		cmns-qtu:BaseUnitn		;n	rdfs:label "gram" ;n	dct:source "https://ucum.org/ucum.html#section-Base-Units" ;n	skos:definition "base unit of mass defined in the Unified Code for Units Of Measure (UCUM) System of Units" ;n	cmns-av:explanatoryNote "The kilogram, as of 2019, is defined by the International Bureau of Weights and Measures from the fixed numerical value of the Planck constant (h), which is 6.62607015×10^−34 kg⋅m^2⋅s^−1" ;n	cmns-av:symbol "g" ;n	cmns-dsg:isDefinedIn cmns-qtu:InternationalSystemOfQuantities ;n	.nnoe2022-iem:HVACn	a owl:Class ;n	rdfs:subClassOfn		oe2022-iem:Equipment ,n		[n			a owl:Restriction ;n			owl:onProperty oe2022-iem:hasState ;n			owl:someValuesFrom oe2022-iem:ThermostatState ;n		]n		;n	rdfs:label "HVAC" ;n	skos:definition "equipment, distribution systems, and terminals that provide, either collectively or individually, the processes of heating, ventilating, or air conditioning to a building or portion of a building" ;n	.nnoe2022-iem:Hourn	an		owl:NamedIndividual ,n		cmns-qtu:ConversionBasedUnit ,n		cmns-qtu:UnitPowerFactorn		;n	rdfs:label "hour" ;n	skos:definition "unit of time representing the 24th part of a day" ;n	cmns-dsg:isDefinedIn cmns-qtu:InternationalSystemOfUnits ;n	cmns-qtu:hasExponent "1/1"^^owl:rational ;n	cmns-qtu:hasMeasurementUnit oe2022-iem:Hour ;n	cmns-qtu:hasQuantityKind oe2022-iem:Time ;n	.nnoe2022-iem:IEQAirQualityEffectn	a owl:Class ;n	rdfs:subClassOfn		oe2022-iem:IEQEffect ,n		[n			a owl:Restriction ;n			owl:onProperty cmns-qtu:hasQuantityValue ;n			owl:someValuesFrom [n				a owl:Restriction ;n				owl:onProperty cmns-qtu:hasMeasurementUnit ;n				owl:someValuesFrom [n					a owl:Restriction ;n					owl:onProperty cmns-qtu:hasQuantityKind ;n					owl:hasValue oe2022-iem:AirQuality ;n				] ;n			] ;n		]n		;n	rdfs:label "indoor environment quality air quality effect" ;n	skos:definition "an air quality effect on the indoor environment quality" ;n	.nnoe2022-iem:IEQAirSpeedEffectn	a owl:Class ;n	rdfs:subClassOfn		oe2022-iem:IEQEffect ,n		[n			a owl:Restriction ;n			owl:onProperty cmns-qtu:hasQuantityValue ;n			owl:someValuesFrom [n				a owl:Restriction ;n				owl:onProperty cmns-qtu:hasMeasurementUnit ;n				owl:someValuesFrom [n					a owl:Restriction ;n					owl:onProperty cmns-qtu:hasQuantityKind ;n					owl:hasValue oe2022-iem:Speed ;n				] ;n			] ;n		]n		;n	rdfs:label "indoor environment quality air speed effect" ;n	skos:definition "an air speed effect on the indoor environment quality" ;n	.nnoe2022-iem:IEQAirTemperatureEffectn	a owl:Class ;n	rdfs:subClassOfn		oe2022-iem:IEQEffect ,n		[n			a owl:Restriction ;n			owl:onProperty cmns-qtu:hasQuantityValue ;n			owl:someValuesFrom [n				a owl:Restriction ;n				owl:onProperty cmns-qtu:hasMeasurementUnit ;n				owl:someValuesFrom [n					a owl:Restriction ;n					owl:onProperty cmns-qtu:hasQuantityKind ;n					owl:hasValue oe2022-iem:Temperature ;n				] ;n			] ;n		]n		;n	rdfs:label "indoor environment quality air temperature effect" ;n	skos:definition "an air temperature effect on the indoor environment quality" ;n	.nnoe2022-iem:IEQEffectn	a owl:Class ;n	rdfs:subClassOf [n		a owl:Restriction ;n		owl:onProperty cmns-qtu:hasQuantityValue ;n		owl:someValuesFrom cmns-qtu:QuantityValue ;n	] ;n	rdfs:label "indoor environment quality effect" ;n	skos:definition "an effect on the indoor environment quality" ;n	.nnoe2022-iem:IEQRelativeHumidityEffectn	a owl:Class ;n	rdfs:subClassOfn		oe2022-iem:IEQEffect ,n		[n			a owl:Restriction ;n			owl:onProperty cmns-qtu:hasQuantityValue ;n			owl:someValuesFrom [n				a owl:Restriction ;n				owl:onProperty cmns-qtu:hasMeasurementUnit ;n				owl:someValuesFrom [n					a owl:Restriction ;n					owl:onProperty cmns-qtu:hasQuantityKind ;n					owl:hasValue oe2022-iem:RelativeHumidity ;n				] ;n			] ;n		]n		;n	rdfs:label "indoor environment quality relative humidity effect" ;n	skos:definition "a relative humidity effect on the indoor environment quality" ;n	.nnoe2022-iem:IndoorAirQualityn	a owl:Class ;n	rdfs:subClassOfn		oe2022-iem:IndoorEnvironmentAttribute ,n		[n			a owl:Restriction ;n			owl:onProperty cmns-qtu:hasQuantityValue ;n			owl:someValuesFrom [n				a owl:Restriction ;n				owl:onProperty cmns-qtu:hasMeasurementUnit ;n				owl:someValuesFrom [n					a owl:Restriction ;n					owl:onProperty cmns-qtu:hasQuantityKind ;n					owl:hasValue oe2022-iem:AirQuality ;n				] ;n			] ;n		]n		;n	rdfs:label "indoor air quality" ;n	skos:definition "an air quality attribute of a local indoor environment" ;n	.nnoe2022-iem:IndoorAirSpeedn	a owl:Class ;n	rdfs:subClassOfn		oe2022-iem:IndoorEnvironmentAttribute ,n		[n			a owl:Restriction ;n			owl:onProperty cmns-qtu:hasQuantityValue ;n			owl:someValuesFrom [n				a owl:Restriction ;n				owl:onProperty cmns-qtu:hasMeasurementUnit ;n				owl:someValuesFrom [n					a owl:Restriction ;n					owl:onProperty cmns-qtu:hasQuantityKind ;n					owl:hasValue oe2022-iem:Speed ;n				] ;n			] ;n		]n		;n	rdfs:label "indoor air speed" ;n	skos:definition "an air speed attribute of a local indoor environment" ;n	.nnoe2022-iem:IndoorAirTemperaturen	a owl:Class ;n	rdfs:subClassOfn		oe2022-iem:IndoorEnvironmentAttribute ,n		[n			a owl:Restriction ;n			owl:onProperty cmns-qtu:hasQuantityValue ;n			owl:someValuesFrom [n				a owl:Restriction ;n				owl:onProperty cmns-qtu:hasMeasurementUnit ;n				owl:someValuesFrom [n					a owl:Restriction ;n					owl:onProperty cmns-qtu:hasQuantityKind ;n					owl:hasValue oe2022-iem:Temperature ;n				] ;n			] ;n		]n		;n	rdfs:label "indoor air temperature" ;n	skos:definition "an air temperature attribute of a local indoor environment" ;n	.nnoe2022-iem:IndoorEnvironmentAttributen	a owl:Class ;n	rdfs:subClassOfn		oe2022-iem:EnvironmentAttribute ,n		[n			a owl:Restriction ;n			owl:onProperty cmns-qtu:hasQuantityValue ;n			owl:onClass cmns-qtu:QuantityValue ;n			owl:maxQualifiedCardinality "1"^^xsd:nonNegativeInteger ;n		]n		;n	rdfs:label "indoor environment" ;n	skos:definition "a quantitative attribute of a local indoor environment" ;n	.nnoe2022-iem:IndoorEnvironmentalQualityn	a owl:Class ;n	rdfs:label "indoor environmental quality" ;n	skos:definition "a perceived indoor experience of the building indoor including thermal comfort, indoor air quality, lighting, acoustics, and control systems" ;n	.nnoe2022-iem:IndoorRelativeHumidityn	a owl:Class ;n	rdfs:subClassOfn		oe2022-iem:IndoorEnvironmentAttribute ,n		[n			a owl:Restriction ;n			owl:onProperty cmns-qtu:hasQuantityValue ;n			owl:someValuesFrom [n				a owl:Restriction ;n				owl:onProperty cmns-qtu:hasMeasurementUnit ;n				owl:someValuesFrom [n					a owl:Restriction ;n					owl:onProperty cmns-qtu:hasQuantityKind ;n					owl:hasValue oe2022-iem:RelativeHumidity ;n				] ;n			] ;n		]n		;n	rdfs:label "indoor relative humidity" ;n	skos:definition "a relative humidity attribute of a local indoor environment" ;n	.nnoe2022-iem:Kelvinn	an		owl:NamedIndividual ,n		cmns-qtu:BaseUnitn		;n	rdfs:label "kelvin" ;n	dct:source "https://ucum.org/ucum.html#section-Base-Units" ;n	rdfs:seeAlso <https://www.nist.gov/pml/owm/si-units-temperature> ;n	skos:definition "base unit of temperature that is defined by taking the fixed numerical value of the Boltzmann constant k to be 1.380 649 ×10^−23 when expressed in the unit J K^−1, which is equal to kg m^2 s^−2 K^−1" ;n	cmns-av:explanatoryNote "The temperature 0 K is commonly referred to as 'absolute zero.' On the widely used Celsius temperature scale, water freezes at 0 °C and boils at about 100 °C. One Celsius degree is an interval of 1 K, and zero degrees Celsius is 273.15 K. An interval of one Celsius degree corresponds to an interval of 1.8 Fahrenheit degrees on the Fahrenheit temperature scale." ;n	cmns-av:symbol "K" ;n	cmns-dsg:isDefinedIn cmns-qtu:InternationalSystemOfUnits ;n	cmns-qtu:hasQuantityKind oe2022-iem:Temperature ;n	.nnoe2022-iem:Kilon	an		owl:NamedIndividual ,n		cmns-qtu:Prefixn		;n	rdfs:label "kilo" ;n	dct:source "https://ucum.org/ucum.html#section-Prefixes" ;n	skos:definition "prefix defined in the Unified Code for Units Of Measure (UCUM) System of Units" ;n	cmns-av:symbol "k" ;n	cmns-dsg:hasDescription "10^3=(10^3)^1" ;n	cmns-dsg:isDefinedIn cmns-qtu:InternationalSystemOfQuantities ;n	.nnoe2022-iem:Kilogramn	an		owl:NamedIndividual ,n		cmns-qtu:PrefixedUnitn		;n	rdfs:label "kilogram" ;n	dct:source "https://ucum.org/ucum.html#section-Base-Units" ;n	rdfs:seeAlso <https://www.nist.gov/si-redefinition/kilogram> ;n	skos:definition "conversion-based unit of mass" ;n	skos:note "Note that in the International System of Units (SI), the kilogram is considered the base unit rather than the gram, which is the base unit in the UCUM." ;n	cmns-av:symbol "kg" ;n	cmns-dsg:hasDescription "10^3 grams" ;n	cmns-dsg:isDefinedIn cmns-qtu:InternationalSystemOfUnits ;n	cmns-qtu:hasFactor oe2022-iem:Kilo ;n	cmns-qtu:hasQuantityKind oe2022-iem:Mass ;n	cmns-qtu:isDerivedFrom oe2022-iem:Gram ;n	.nnoe2022-iem:Kilowattn	an		owl:NamedIndividual ,n		cmns-qtu:PrefixedUnitn		;n	rdfs:label "kilowatt" ;n	skos:definition "conversion-based unit of energy" ;n	cmns-dsg:isDefinedIn cmns-qtu:InternationalSystemOfUnits ;n	cmns-qtu:hasFactor oe2022-iem:Kilo ;n	cmns-qtu:hasQuantityKind oe2022-iem:Energy ;n	cmns-qtu:isDerivedFrom oe2022-iem:Watt ;n	.nnoe2022-iem:KilowattHourn	an		owl:NamedIndividual ,n		cmns-qtu:DerivedUnitn		;n	rdfs:label "kilowatt-hour" ;n	skos:definition "measure of electrical energy equivalent to a power consumption of 1,000 watts for 1 hour" ;n	cmns-dsg:isDefinedIn cmns-qtu:InternationalSystemOfUnits ;n	cmns-qtu:hasFactor oe2022-iem:Hour ;n	cmns-qtu:hasQuantityKind oe2022-iem:Energy ;n	cmns-qtu:isDerivedFrom oe2022-iem:Kilowatt ;n	.nnoe2022-iem:Lengthn	an		owl:NamedIndividual ,n		cmns-qtu:BaseQuantityKindn		;n	rdfs:label "length" ;n	dct:source "https://ucum.org/ucum.html#section-Base-Units" ;n	skos:definition "base quantity kind that is the quantitative measure of distance, i.e., of how far apart objects or points are" ;n	cmns-av:symbol "l" ;n	cmns-dsg:isDefinedIn cmns-qtu:InternationalSystemOfQuantities ;n	.nnoe2022-iem:Massn	an		owl:NamedIndividual ,n		cmns-qtu:BaseQuantityKindn		;n	rdfs:label "mass" ;n	skos:definition "base quantity kind for the measure of a measure of a body's inertial property or how much matter it contains" ;n	cmns-av:explanatoryNote "Note that as of 2018, mass has been redefined in the International System of Units in terms of Planck's constant, h. The kilogram is defined by taking the fixed numerical value of the Planck constant, h, to be 6.626 070 15 × 10-34 when expressed in the unit J s, which is equal to kg m^2 s^−1, where the metre and the second are defined in terms of the speed of light, 𝒸, and the hyperfine transition frequency of the caesium-133 atom, ∆ν, respectively." ;n	cmns-av:symbol "m" ;n	cmns-dsg:isDefinedIn cmns-qtu:InternationalSystemOfQuantities ;n	.nnoe2022-iem:Metern	an		owl:NamedIndividual ,n		cmns-qtu:BaseUnitn		;n	rdfs:label "meter" ;n	dct:source "https://ucum.org/ucum.html#section-Base-Units" ;n	rdfs:seeAlson		<https://www.nist.gov/pml/owm/si-units-length> ,n		<https://www.nist.gov/system/files/documents/pml/div683/museum-length.pdf>n		;n	skos:definition "base unit of length that is the distance traveled by light in vacuum during the time interval of 1/299 792 458 of a second" ;n	cmns-av:symbol "m" ;n	cmns-dsg:isDefinedIn cmns-qtu:InternationalSystemOfUnits ;n	cmns-qtu:hasQuantityKind oe2022-iem:Length ;n	.nnoe2022-iem:MetersPerSecondn	an		owl:NamedIndividual ,n		cmns-qtu:DerivedUnitn		;n	rdfs:label "meter per second" ;n	skos:definition "measure of speed equipvalent to the moved meters for 1 second" ;n	cmns-dsg:isDefinedIn cmns-qtu:InternationalSystemOfUnits ;n	cmns-qtu:hasFactor oe2022-iem:PerSecond ;n	cmns-qtu:hasQuantityKind oe2022-iem:Speed ;n	cmns-qtu:isDerivedFrom oe2022-iem:Meter ;n	.nnoe2022-iem:Occupantn	a owl:Class ;n	rdfs:subClassOfn		cmns-pts:PartyRole ,n		[n			a owl:Restriction ;n			owl:onProperty cmns-pts:isPlayedBy ;n			owl:onClass oe2022-iem:Person ;n			owl:qualifiedCardinality "1"^^xsd:nonNegativeInteger ;n		]n		;n	rdfs:label "occupant"@en ;n	skos:definition "someone that resides or is present in or using a building, vehicle, seat, place, etc., at a given time"@en ;n	.nnoe2022-iem:OffStaten	a owl:Class ;n	rdfs:subClassOf oe2022-iem:ComponentState ;n	rdfs:label "off state" ;n	skos:definition "condition of not being activated" ;n	.nnoe2022-iem:OnStaten	a owl:Class ;n	rdfs:subClassOf oe2022-iem:ComponentState ;n	rdfs:label "on state" ;n	skos:definition "condition of being currently in operation" ;n	.nnoe2022-iem:OpenStaten	a owl:Class ;n	rdfs:subClassOf oe2022-iem:ComponentState ;n	rdfs:label "open state" ;n	skos:definition "condition of being not closed" ;n	.nnoe2022-iem:Organizationn	a owl:Class ;n	rdfs:subClassOf cmns-pts:Party ;n	rdfs:label "organization"@en ;n	rdfs:seeAlso <https://www.w3.org/TR/vocab-org/#org:Organization> ;n	skos:definition "collection of one or more people, or groups of people formed together into a community or other social, commercial or political structure to act, or that is designated to act, towards some purpose, such as to meet a need or pursue collective goals on a continuing basis"@en ;n	skos:example "This may be a business entity, government, international organization, not-for-profit, academic institution, or other unincorporated and/or informal social organization."@en ;n	cmns-av:adaptedFrom "https://www.iso.org/obp/ui/#iso:std:iso-iec:6523:-1:ed-1:v1:en" ;n	.nnoe2022-iem:OutdoorAirQualityn	a owl:Class ;n	rdfs:subClassOfn		oe2022-iem:OutdoorEnvironmentAttribute ,n		[n			a owl:Restriction ;n			owl:onProperty cmns-qtu:hasQuantityValue ;n			owl:someValuesFrom [n				a owl:Restriction ;n				owl:onProperty cmns-qtu:hasMeasurementUnit ;n				owl:someValuesFrom [n					a owl:Restriction ;n					owl:onProperty cmns-qtu:hasQuantityKind ;n					owl:hasValue oe2022-iem:AirQuality ;n				] ;n			] ;n		]n		;n	rdfs:label "outdoor air quality" ;n	skos:definition "an air quality attribute of a local outdoor environment" ;n	.nnoe2022-iem:OutdoorAirSpeedn	a owl:Class ;n	rdfs:subClassOfn		oe2022-iem:OutdoorEnvironmentAttribute ,n		[n			a owl:Restriction ;n			owl:onProperty cmns-qtu:hasQuantityValue ;n			owl:someValuesFrom [n				a owl:Restriction ;n				owl:onProperty cmns-qtu:hasMeasurementUnit ;n				owl:someValuesFrom [n					a owl:Restriction ;n					owl:onProperty cmns-qtu:hasQuantityKind ;n					owl:hasValue oe2022-iem:Speed ;n				] ;n			] ;n		]n		;n	rdfs:label "outdoor air speed" ;n	skos:definition "an air speed attribute of a local outdoor environment" ;n	.nnoe2022-iem:OutdoorAirTemperaturen	a owl:Class ;n	rdfs:subClassOfn		oe2022-iem:OutdoorEnvironmentAttribute ,n		[n			a owl:Restriction ;n			owl:onProperty cmns-qtu:hasQuantityValue ;n			owl:someValuesFrom [n				a owl:Restriction ;n				owl:onProperty cmns-qtu:hasMeasurementUnit ;n				owl:someValuesFrom [n					a owl:Restriction ;n					owl:onProperty cmns-qtu:hasQuantityKind ;n					owl:hasValue oe2022-iem:Temperature ;n				] ;n			] ;n		]n		;n	rdfs:label "outdoor air temperature" ;n	skos:definition "an air temperature attribute of a local outdoor environment" ;n	.nnoe2022-iem:OutdoorDaylightIntensityn	a owl:Class ;n	rdfs:subClassOf oe2022-iem:OutdoorEnvironmentAttribute ;n	rdfs:label "outdoor daylight intensity" ;n	skos:definition "a daylight intensity attribute of a local outdoor environment" ;n	.nnoe2022-iem:OutdoorEnvironmentAttributen	a owl:Class ;n	rdfs:subClassOfn		oe2022-iem:EnvironmentAttribute ,n		[n			a owl:Restriction ;n			owl:onProperty cmns-qtu:hasQuantityValue ;n			owl:onClass cmns-qtu:QuantityValue ;n			owl:maxQualifiedCardinality "1"^^xsd:nonNegativeInteger ;n		]n		;n	rdfs:label "outdoor environment" ;n	skos:definition "a quantitative attribute of a local outdoor environment" ;n	.nnoe2022-iem:OutdoorRelativeHumidityn	a owl:Class ;n	rdfs:subClassOfn		oe2022-iem:OutdoorEnvironmentAttribute ,n		[n			a owl:Restriction ;n			owl:onProperty oe2022-iem:hasEffect ;n			owl:someValuesFrom oe2022-iem:IEQRelativeHumidityEffect ;n		] ,n		[n			a owl:Restriction ;n			owl:onProperty cmns-qtu:hasQuantityValue ;n			owl:someValuesFrom [n				a owl:Restriction ;n				owl:onProperty cmns-qtu:hasMeasurementUnit ;n				owl:someValuesFrom [n					a owl:Restriction ;n					owl:onProperty cmns-qtu:hasQuantityKind ;n					owl:hasValue oe2022-iem:RelativeHumidity ;n				] ;n			] ;n		]n		;n	rdfs:label "outdoor relative humidity" ;n	skos:definition "a relative humidity attribute of a local outdoor environment" ;n	.nnoe2022-iem:PerCubicSecondn	an		owl:NamedIndividual ,n		cmns-qtu:UnitPowerFactorn		;n	cmns-qtu:hasExponent "-3/1"^^owl:rational ;n	cmns-qtu:hasMeasurementUnit oe2022-iem:Second ;n	.nnoe2022-iem:PerCubicTimen	an		owl:NamedIndividual ,n		cmns-qtu:QuantityKindPowerFactorn		;n	cmns-qtu:hasExponent "-3/1"^^owl:rational ;n	cmns-qtu:hasQuantityKind oe2022-iem:Time ;n	.nnoe2022-iem:PerHourn	an		owl:NamedIndividual ,n		cmns-qtu:UnitPowerFactorn		;n	cmns-qtu:hasExponent "-1/1"^^owl:rational ;n	cmns-qtu:hasMeasurementUnit oe2022-iem:Hour ;n	.nnoe2022-iem:PerSecondn	an		owl:NamedIndividual ,n		cmns-qtu:UnitPowerFactorn		;n	cmns-qtu:hasExponent "-1/1"^^owl:rational ;n	cmns-qtu:hasMeasurementUnit oe2022-iem:Second ;n	.nnoe2022-iem:PerTimen	an		owl:NamedIndividual ,n		cmns-qtu:QuantityKindPowerFactorn		;n	cmns-qtu:hasExponent "-1/1"^^owl:rational ;n	cmns-qtu:hasQuantityKind oe2022-iem:Time ;n	.nnoe2022-iem:Personn	a owl:Class ;n	rdfs:subClassOf cmns-pts:Party ;n	rdfs:label "person"@en ;n	skos:definition "individual human being, with consciousness of self"@en ;n	cmns-av:synonym "natural person"@en ;n	.nnoe2022-iem:Radiatorn	a owl:Class ;n	rdfs:subClassOfn		oe2022-iem:Equipment ,n		[n			a owl:Restriction ;n			owl:onProperty oe2022-iem:hasState ;n			owl:allValuesFrom [n				a owl:Class ;n				owl:unionOf (n					oe2022-iem:OffStaten					oe2022-iem:OnStaten				) ;n			] ;n		]n		;n	rdfs:label "radiator" ;n	skos:definition "HVAC equipment that can raise the indoor temperature by transferring heat from an internal system into a room" ;n	.nnoe2022-iem:RelativeHumidityn	an		owl:NamedIndividual ,n		cmns-qtu:DimensionlessQuantityn		;n	rdfs:label "relatvie humidity" ;n	skos:definition "ratio of the mole fraction of water vapor to the mole fraction of water vapor saturated at the same temperature and barometric pressure." ;n	.nnoe2022-iem:Roomn	a owl:Class ;n	rdfs:label "room" ;n	skos:definition "region in a building in which occupant comfort and measurements apply" ;n	.nnoe2022-iem:RoomComponentn	a owl:Class ;n	rdfs:label "room component" ;n	skos:definition "an object in a room that can be used to alter relevant IEQ parameters" ;n	.nnoe2022-iem:Secondn	an		owl:NamedIndividual ,n		cmns-qtu:BaseUnitn		;n	cmns-dsg:isDefinedIn cmns-qtu:InternationalSystemOfUnits ;n	cmns-qtu:hasQuantityKind oe2022-iem:Time ;n	.nnoe2022-iem:Speedn	an		owl:NamedIndividual ,n		cmns-qtu:DerivedQuantityKindn		;n	cmns-dsg:isDefinedIn cmns-qtu:InternationalSystemOfQuantities ;n	cmns-qtu:hasFactor oe2022-iem:PerTime ;n	.nnoe2022-iem:SquareLengthn	an		owl:NamedIndividual ,n		cmns-qtu:QuantityKindPowerFactorn		;n	cmns-qtu:hasExponent "2/1"^^owl:rational ;n	cmns-qtu:hasQuantityKind oe2022-iem:Length ;n	.nnoe2022-iem:SquareMetern	an		owl:NamedIndividual ,n		cmns-qtu:UnitPowerFactorn		;n	cmns-qtu:hasExponent "2/1"^^owl:rational ;n	cmns-qtu:hasMeasurementUnit oe2022-iem:Meter ;n	.nnoe2022-iem:Temperaturen	an		owl:NamedIndividual ,n		cmns-qtu:BaseQuantityKindn		;n	rdfs:label "temperature" ;n	dct:source "https://ucum.org/ucum.html#section-Base-Units" ;n	skos:definition "base quantity kind that is the quantitative measure of the ability of a substance, or more generally of any physical system, to transfer heat energy to another physical system" ;n	cmns-av:explanatoryNote "There are three types of temperature scale: those, such as the SI scale, that are defined in terms of the average translational kinetic energy per freely moving microscopic particle, such as atom, molecule, or electron, in a body; those that rely solely on purely macroscopic properties and thermodynamic principles, such as Kelvin's original definition; and those that are not defined by theoretical principles, but are defined by convenient empirical properties of particular materials." ;n	cmns-av:symbol "T" ;n	cmns-dsg:isDefinedIn cmns-qtu:InternationalSystemOfQuantities ;n	.nnoe2022-iem:ThermalComfortn	a owl:Class ;n	rdfs:subClassOf oe2022-iem:IndoorEnvironmentalQuality ;n	rdfs:label "thermal comfort" ;n	skos:definition "the condition of mind which expresses satisfaction with the surrounding thermal environment and is assessed by subjective evaluation" ;n	.nnoe2022-iem:ThermostatStaten	a owl:Class ;n	rdfs:subClassOfn		oe2022-iem:ComponentState ,n		[n			a owl:Restriction ;n			owl:onProperty cmns-qtu:hasQuantityValue ;n			owl:someValuesFrom [n				a owl:Class ;n				owl:intersectionOf (n					cmns-qtu:QuantityValuen					[n						a owl:Restriction ;n						owl:onProperty cmns-qtu:hasMeasurementUnit ;n						owl:someValuesFrom [n							a owl:Restriction ;n							owl:onProperty cmns-qtu:hasQuantityKind ;n							owl:hasValue oe2022-iem:Temperature ;n						] ;n					]n				) ;n			] ;n		]n		;n	rdfs:label "thermostat state" ;n	skos:definition "numeric value at which the thermostat is set" ;n	.nnoe2022-iem:Timen	an		owl:NamedIndividual ,n		cmns-qtu:BaseQuantityKindn		;n	cmns-dsg:isDefinedIn cmns-qtu:InternationalSystemOfQuantities ;n	.nnoe2022-iem:Wattn	an		owl:NamedIndividual ,n		cmns-qtu:DerivedUnitn		;n	rdfs:label "watt" ;n	skos:definition "unit of power equivalent to one joule per second" ;n	cmns-dsg:isDefinedIn cmns-qtu:InternationalSystemOfQuantities ;n	cmns-qtu:hasFactorn		oe2022-iem:PerCubicSecond ,n		oe2022-iem:SquareMetern		;n	cmns-qtu:hasQuantityKind oe2022-iem:Work ;n	cmns-qtu:isDerivedFrom oe2022-iem:Kilogram ;n	.nnoe2022-iem:Windown	a owl:Class ;n	rdfs:subClassOf oe2022-iem:Furniture ;n	rdfs:label "window" ;n	owl:disjointWith oe2022-iem:WindowBlinds ;n	skos:definition "room component that can optionally let air flow between inside and outside regions" ;n	.nnoe2022-iem:WindowBlindsn	a owl:Class ;n	rdfs:subClassOf oe2022-iem:Furniture ;n	rdfs:label "window blinds" ;n	skos:definition "room component that be open or closed, thereby letting in or blocking light, respectively" ;n	.nnoe2022-iem:Workn	an		owl:NamedIndividual ,n		cmns-qtu:DerivedQuantityKindn		;n	cmns-dsg:isDefinedIn cmns-qtu:InternationalSystemOfQuantities ;n	cmns-qtu:hasFactorn		oe2022-iem:PerCubicTime ,n		oe2022-iem:SquareLengthn		;n	.nnoe2022-iem:hasAttributen	a owl:ObjectProperty ;n	rdfs:subPropertyOf owl:topObjectProperty ;n	rdfs:label "has attribute" ;n	owl:inverseOf oe2022-iem:isAttributeOf ;n	skos:definition "has components that affect the nature of the whole with respect to relevant actors" ;n	.nnoe2022-iem:hasEffectn	a owl:ObjectProperty ;n	rdfs:label "has effect" ;n	skos:definition "specify how to achange the parameters of indoor environmental quality" ;n	.nnoe2022-iem:hasPossibleStaten	a owl:ObjectProperty ;n	rdfs:subPropertyOf owl:topObjectProperty ;n	rdfs:label "has possible state" ;n	rdfs:domain oe2022-iem:RoomComponent ;n	rdfs:range oe2022-iem:ComponentState ;n	owl:inverseOf oe2022-iem:isPossibleStateOf ;n	skos:definition "has the ability to be in some condition at a point in time" ;n	.nnoe2022-iem:hasStaten	a owl:ObjectProperty ;n	rdfs:subPropertyOf owl:topObjectProperty ;n	rdfs:label "has state" ;n	rdfs:domain oe2022-iem:RoomComponent ;n	rdfs:range oe2022-iem:ComponentState ;n	owl:inverseOf oe2022-iem:isStateOf ;n	skos:definition "is currently in the condition, referring to objects that have some changeable condition" ;n	.nnoe2022-iem:isAttributeOfn	a owl:ObjectProperty ;n	rdfs:subPropertyOf owl:topObjectProperty ;n	rdfs:label "is attribute of" ;n	skos:definition "is a component that affects the nature of the whole with respect to relevant actors" ;n	.nnoe2022-iem:isPossibleStateOfn	a owl:ObjectProperty ;n	rdfs:subPropertyOf owl:topObjectProperty ;n	rdfs:label "is possible state of" ;n	skos:definition "can be the condition of a given object at some point in time" ;n	.nnoe2022-iem:isQuantifiedByn	a owl:ObjectProperty ;n	rdfs:label "is quantified by" ;n	owl:inverseOf oe2022-iem:quatifies ;n	skos:definition "is specified by the quantify of the object" ;n	.nnoe2022-iem:isStateOfn	a owl:ObjectProperty ;n	rdfs:subPropertyOf owl:topObjectProperty ;n	rdfs:labeln		"is currently the condition of" ,n		"is state of"n		;n	.nnoe2022-iem:quatifiesn	a owl:ObjectProperty ;n	rdfs:label "quantifies" ;n	skos:definition "specifies the quantify of the object" ;n	.nn[]n	a owl:AllDisjointClasses ;n	owl:members (n		oe2022-iem:ClosedStaten		oe2022-iem:OffStaten		oe2022-iem:OnStaten		oe2022-iem:OpenStaten	) ;n	.nn[]n	a owl:AllDisjointClasses ;n	owl:members (n		oe2022-iem:Dehumidifiern		oe2022-iem:Fann		oe2022-iem:HVACn		oe2022-iem:Radiatorn	) ;n	.nn[]n	a owl:AllDisjointClasses ;n	owl:members (n		oe2022-iem:IEQAirQualityEffectn		oe2022-iem:IEQAirSpeedEffectn		oe2022-iem:IEQAirTemperatureEffectn		oe2022-iem:IEQRelativeHumidityEffectn	) ;n	.nn[]n	a owl:AllDisjointClasses ;n	owl:members (n		oe2022-iem:IndoorAirQualityn		oe2022-iem:IndoorAirSpeedn		oe2022-iem:IndoorAirTemperaturen		oe2022-iem:IndoorRelativeHumidityn	) ;n	.nn[]n	a owl:AllDisjointClasses ;n	owl:members (n		oe2022-iem:OffStaten		oe2022-iem:OnStaten		oe2022-iem:OpenStaten		oe2022-iem:ThermostatStaten	) ;n	.nn[]n	a owl:AllDisjointClasses ;n	owl:members (n		oe2022-iem:OutdoorAirQualityn		oe2022-iem:OutdoorAirSpeedn		oe2022-iem:OutdoorAirTemperaturen		oe2022-iem:OutdoorDaylightIntensityn		oe2022-iem:OutdoorRelativeHumidityn	) ;n	.nn